lists, verified but bare and missing some stuff

compiler/scheme/proofs/scheme_to_cakeProofScript.sml
@@ -45,7 +45,9 @@ Theorem scheme_cons_env_def[allow_rebind, compute] = EVAL_RULE $ zDefine ‘
 Theorem scheme_env_app_def[allow_rebind, compute] = EVAL_RULE $ zDefine ‘
   scheme_env_app env <=>
     env.c = scheme_cons_env ∧
-    EVERY (λ dec. ∃ env_cl . env_cl.c = scheme_cons_env ∧ closure_in_env env dec env_cl) scheme_basis
+    EVERY (λ dec. ∃ env_cl . env_cl.c = scheme_cons_env ∧ closure_in_env env dec env_cl) (TAKE 2 scheme_basis ++ DROP 3 scheme_basis) /\
+    (? env_sminus . env_sminus.c = scheme_cons_env /\ closure_in_env env (EL 2 scheme_basis) env_sminus /\
+      (? env_sadd . env_sadd.c = scheme_cons_env /\ closure_in_env env_sminus (EL 0 scheme_basis) env_sadd))
 ’;
 
 Theorem scheme_env_def[allow_rebind, compute] = RESTR_EVAL_RULE [``scheme_env_app``] $ zDefine ‘
@@ -75,8 +77,8 @@ Proof
               | (st', Rval env) => env’
   >> EVAL_TAC
   >> rpt strip_tac
-  >> irule_at (Pos last) EQ_REFL
-  >> simp[]
+  >> irule_at Any EQ_REFL
+  >> simp[nsLookup_def]
 QED
 
 (*
@@ -118,147 +120,12 @@ Theorem scheme_typestamp_def[allow_rebind, simp, compute] = SRULE [] $
       scheme_conses_def, SND, THE_DEF, nsLookup_def, scheme_cons_env_def]
     “EVERY (λ x . scheme_typestamp x = scheme_typestamp x) scheme_conses”;
 
-Definition muts_loc_def:
-  muts_loc nl [] l = nl + l /\
-  muts_loc nl (Refv _::refs) 0 = nl /\
-  muts_loc nl (Refv _::refs) (SUC l) = muts_loc (SUC nl) refs l /\
-  muts_loc nl (_::refs) l = muts_loc (SUC nl) refs l
-End
-
-Theorem muts_loc_props:
-  ! nl refs l . muts_loc nl refs l >= nl + l /\ muts_loc (SUC nl) refs l = SUC (muts_loc nl refs l)
-Proof
-  ho_match_mp_tac muts_loc_ind
-  >> simp[muts_loc_def]
-QED
-
-Theorem muts_loc_mono = cj 1 muts_loc_props;
-Theorem muts_loc_SUC[simp] = cj 2 muts_loc_props;
-
-Theorem muts_loc_FILTER:
-  ! refs l .
-    (muts_loc 0 refs l < LENGTH refs
-     <=> l < LENGTH (FILTER (\ref. case ref of | Refv _ => T | _ => F) refs))
-    /\
-    EL (muts_loc 0 refs l) refs
-     = EL l $ FILTER (\ref. case ref of | Refv _ => T | _ => F) refs
-Proof
-  Induct >> Induct
-  >> simp[muts_loc_def]
-  >> gen_tac >> Cases
-  >> simp[muts_loc_def]
-QED
-
-Theorem muts_loc_alloc_same:
-  ! refs l mlv .
-    muts_loc 0 refs l = muts_loc 0 (refs ++ [Refv mlv]) l
-Proof
-  Induct >> Induct
-  >> simp[muts_loc_def]
-  >> gen_tac >> Cases
-  >> simp[muts_loc_def]
-QED
-
-Theorem muts_loc_LUPDATE_same:
-  ! refs l l' mlv mlv' .
-    EL l' refs = Refv mlv
-    ==>
-    muts_loc 0 refs l = muts_loc 0 (LUPDATE (Refv mlv') l' refs) l
-Proof
-  Induct >> Induct
-  >> simp[muts_loc_def, LUPDATE_def] >- (
-    gen_tac >> Cases >> Cases
-    >> simp[muts_loc_def, LUPDATE_def]
-  )
-  >> gen_tac >> gen_tac >> Cases
-  >> simp[muts_loc_def, LUPDATE_def]
-QED
-
-Definition pairs_loc_def:
-  pairs_loc nl [] l = nl + l /\
-  pairs_loc nl (Varray _::refs) 0 = nl /\
-  pairs_loc nl (Varray _::refs) (SUC l) = pairs_loc (SUC nl) refs l /\
-  pairs_loc nl (_::refs) l = pairs_loc (SUC nl) refs l
-End
-
-Theorem pairs_loc_props:
-  ! nl refs l . pairs_loc nl refs l >= nl + l /\ pairs_loc (SUC nl) refs l = SUC (pairs_loc nl refs l)
-Proof
-  ho_match_mp_tac pairs_loc_ind
-  >> simp[pairs_loc_def]
-QED
-
-Theorem pairs_loc_mono = cj 1 pairs_loc_props;
-Theorem pairs_loc_SUC[simp] = cj 2 pairs_loc_props;
-
-Theorem pairs_loc_FILTER:
-  ! refs l .
-    (pairs_loc 0 refs l < LENGTH refs
-     <=> l < LENGTH (FILTER (\ref. case ref of | Varray _ => T | _ => F) refs))
-    /\
-    EL (pairs_loc 0 refs l) refs
-     = EL l $ FILTER (\ref. case ref of | Varray _ => T | _ => F) refs
-Proof
-  Induct >> Induct
-  >> simp[pairs_loc_def]
-  >> gen_tac >> Cases
-  >> simp[pairs_loc_def]
-QED
-
-Theorem pairs_loc_alloc_diff:
-  ! refs l mlv .
-    pairs_loc 0 refs l < LENGTH refs ==> pairs_loc 0 refs l = pairs_loc 0 (refs ++ [Refv mlv]) l
-Proof
-  Induct >> Induct
-  >> simp[pairs_loc_def]
-  >> gen_tac >> Cases
-  >> simp[pairs_loc_def]
-QED
-
-Theorem pairs_loc_LUPDATE_diff:
-  ! refs l l' mlv mlv' .
-    EL l' refs = Refv mlv
-    ==>
-    pairs_loc 0 refs l = pairs_loc 0 (LUPDATE (Refv mlv') l' refs) l
-Proof
-  Induct >> Induct
-  >> simp[pairs_loc_def, LUPDATE_def]
-  >> gen_tac >> Cases >> Cases
-  >> simp[pairs_loc_def, LUPDATE_def]
-QED
-
 Inductive env_rel:
-  FEVERY (λ (x, n).
-    nsLookup env.v (Short ("var" ++ explode x)) = SOME (Loc T (muts_loc 0 refs n))) se
+  FEVERY (λ (x, l).
+    nsLookup env.v (Short ("var" ++ explode x)) = SOME (Loc T l)) se
   ⇒
-  env_rel refs se env
+  env_rel se env
 End
-
-Theorem env_rel_alloc:
-  ! refs mlv se env .
-    env_rel refs se env ==> env_rel (refs ++ [Refv mlv]) se env
-Proof
-  simp[env_rel_cases]
-  >> rpt strip_tac
-  >> irule FEVERY_MONO
-  >> pop_assum $ irule_at $ Pos last
-  >> PairCases
-  >> simp[muts_loc_alloc_same]
-QED
-
-Theorem env_rel_LUPDATE_same:
-  ! refs l mlv'1 mlv'2 se env .
-    EL l refs = Refv mlv'1
-    ==>
-    env_rel refs se env ==> env_rel (LUPDATE (Refv mlv'2) l refs) se env
-Proof
-  simp[env_rel_cases]
-  >> rpt strip_tac
-  >> irule FEVERY_MONO
-  >> pop_assum $ irule_at $ Pos last
-  >> PairCases
-  >> rw[muts_loc_LUPDATE_same]
-QED
 
 Theorem vcons_list_def[allow_rebind] = SRULE [] $ Define ‘
   vcons_list [] = Conv (SOME (scheme_typestamp "[]")) [] ∧
@@ -276,144 +143,142 @@ End
 
 Inductive val_cont_rels:
 [~SBool_T:]
-  ml_v_vals refs (SBool T) $
+  ml_v_vals (SBool T) $
     Conv (SOME (scheme_typestamp "SBool")) [Conv (SOME (scheme_typestamp "True")) []]
 [~SBool_F:]
-  ml_v_vals refs (SBool F) $
+  ml_v_vals (SBool F) $
     Conv (SOME (scheme_typestamp "SBool")) [Conv (SOME (scheme_typestamp "False")) []]
 [~SNum:]
-  ml_v_vals refs (SNum i) $
+  ml_v_vals (SNum i) $
     Conv (SOME (scheme_typestamp "SNum")) [Litv (IntLit i)]
 [~Prim_SAdd:]
-  ml_v_vals refs (Prim SAdd) $
+  ml_v_vals (Prim SAdd) $
     Conv (SOME (scheme_typestamp "Prim")) [Conv (SOME (scheme_typestamp "SAdd")) []]
 [~Prim_SMul:]
-  ml_v_vals refs (Prim SMul) $
+  ml_v_vals (Prim SMul) $
     Conv (SOME (scheme_typestamp "Prim")) [Conv (SOME (scheme_typestamp "SMul")) []]
 [~Prim_SMinus:]
-  ml_v_vals refs (Prim SMinus) $
+  ml_v_vals (Prim SMinus) $
     Conv (SOME (scheme_typestamp "Prim")) [Conv (SOME (scheme_typestamp "SMinus")) []]
 [~Prim_SEqv:]
-  ml_v_vals refs (Prim SEqv) $
+  ml_v_vals (Prim SEqv) $
     Conv (SOME (scheme_typestamp "Prim")) [Conv (SOME (scheme_typestamp "SEqv")) []]
 [~Prim_CallCC:]
-  ml_v_vals refs (Prim CallCC) $
+  ml_v_vals (Prim CallCC) $
     Conv (SOME (scheme_typestamp "Prim")) [Conv (SOME (scheme_typestamp "CallCC")) []]
 [~Prim_Cons:]
-  ml_v_vals refs (Prim Cons) $
+  ml_v_vals (Prim Cons) $
     Conv (SOME (scheme_typestamp "Prim")) [Conv (SOME (scheme_typestamp "Cons")) []]
 [~Prim_Car:]
-  ml_v_vals refs (Prim Car) $
+  ml_v_vals (Prim Car) $
     Conv (SOME (scheme_typestamp "Prim")) [Conv (SOME (scheme_typestamp "Car")) []]
 [~Prim_Cdr:]
-  ml_v_vals refs (Prim Cdr) $
+  ml_v_vals (Prim Cdr) $
     Conv (SOME (scheme_typestamp "Prim")) [Conv (SOME (scheme_typestamp "Cdr")) []]
 [~Prim_Wrong:]
-  ml_v_vals refs (Wrong s) $
+  ml_v_vals (Wrong s) $
     Conv (SOME (scheme_typestamp "Wrong")) [Litv (StrLit s)]
 [~Proc:]
   scheme_env env ∧
-  env_rel refs se env ∧
+  env_rel se env ∧
   ce = cps_transform e ∧
   inner = proc_ml xs xp "k" ce
   ⇒
-  ml_v_vals refs (Proc se xs xp e) $
+  ml_v_vals (Proc se xs xp e) $
     Conv (SOME (scheme_typestamp "Proc")) [
       Closure env "k" $ Fun "ts" inner
     ]
 [~Throw:]
-  cont_rel refs ks kv
+  cont_rel ks kv
   ⇒
-  ml_v_vals refs (Throw ks) $
+  ml_v_vals (Throw ks) $
     Conv (SOME (scheme_typestamp "Throw")) [kv]
 [~SList:]
-  LIST_REL (ml_v_vals refs) vs mlvs
+  LIST_REL ml_v_vals vs mlvs
   ⇒
-  ml_v_vals refs (SList vs) $
+  ml_v_vals (SList vs) $
     Conv (SOME (scheme_typestamp "SList")) [vcons_list mlvs]
 [~PairP:]
-  pairs_loc 0 refs l < LENGTH refs
-  ⇒
-  ml_v_vals refs (PairP l) $
-    Conv (SOME (scheme_typestamp "PairP")) [Loc T (pairs_loc 0 refs l)]
+  ml_v_vals (PairP l) $
+    Conv (SOME (scheme_typestamp "PairP")) [Loc T l]
 [~Nul:]
-  ml_v_vals refs Null $
+  ml_v_vals Null $
     Conv (SOME (scheme_typestamp "Null")) []
 
 [~Id:]
   scheme_env env
   ⇒
-  cont_rel refs []
+  cont_rel []
     (Closure env "t" (Var (Short "t")))
 [~CondK:]
-  cont_rel refs ks kv ∧
+  cont_rel ks kv ∧
   nsLookup env.v (Short "k") = SOME kv ∧
   ct = cps_transform te ∧
   cf = cps_transform fe ∧
   scheme_env env ∧
-  env_rel refs se env
+  env_rel se env
   ⇒
-  cont_rel refs ((se, CondK te fe) :: ks)
+  cont_rel ((se, CondK te fe) :: ks)
     (Closure env "t" $ Mat (Var (Short "t")) [
       (Pcon (SOME $ Short "SBool") [Pcon (SOME $ Short "False") []],
         App Opapp [cf; Var (Short "k")]);
       (Pany, App Opapp [ct;  Var (Short "k")])
     ])
 [~ApplyK_NONE:]
-  cont_rel refs ks kv ∧
+  cont_rel ks kv ∧
   nsLookup env.v (Short "k") = SOME kv ∧
   inner = cps_transform_app (Var (Short "t")) [] es (Var (Short "k")) ∧
   scheme_env env ∧
-  env_rel refs se env
+  env_rel se env
   ⇒
-  cont_rel refs ((se, ApplyK NONE es) :: ks)
+  cont_rel ((se, ApplyK NONE es) :: ks)
     (Closure env "t" $ inner)
 [~ApplyK_SOME:]
-  cont_rel refs ks kv ∧
+  cont_rel ks kv ∧
   nsLookup env.v (Short "k") = SOME kv ∧
   (t, ts) = cps_app_ts vs ∧
   inner = cps_transform_app (Var (Short "t"))
     (MAP (Var o Short) (t::ts)) es (Var (Short "k")) ∧
-  ml_v_vals refs fn mlfn ∧
+  ml_v_vals fn mlfn ∧
   nsLookup env.v (Short "t") = SOME mlfn ∧
-  LIST_REL (ml_v_vals refs) vs mlvs ∧
+  LIST_REL ml_v_vals vs mlvs ∧
   LIST_REL (λ x mlv . nsLookup env.v (Short x) = SOME mlv) ts mlvs ∧
   scheme_env env ∧
-  env_rel refs se env
+  env_rel se env
   ⇒
-  cont_rel refs ((se, ApplyK (SOME (fn, vs)) es) :: ks)
+  cont_rel ((se, ApplyK (SOME (fn, vs)) es) :: ks)
     (Closure env t $ inner)
 [~BeginK:]
-  cont_rel refs ks kv ∧
+  cont_rel ks kv ∧
   nsLookup env.v (Short "k") = SOME kv ∧
   inner = cps_transform_seq (Var (Short "k")) es e ∧
   scheme_env env ∧
-  env_rel refs se env
+  env_rel se env
   ⇒
-  cont_rel refs ((se, BeginK es e) :: ks)
+  cont_rel ((se, BeginK es e) :: ks)
     (Closure env "_" $ inner)
 [~SetK:]
-  cont_rel refs ks kv ∧
+  cont_rel ks kv ∧
   nsLookup env.v (Short "k") = SOME kv ∧
   inner = refunc_set (Var (Short "t")) (Var (Short "k")) x ∧
   scheme_env env ∧
-  env_rel refs se env
+  env_rel se env
   ⇒
-  cont_rel refs ((se, SetK x) :: ks)
+  cont_rel ((se, SetK x) :: ks)
     (Closure env "t" $ inner)
 [~LetinitK:]
-  cont_rel refs ks kv ∧
+  cont_rel ks kv ∧
   nsLookup env.v (Short "k") = SOME kv ∧
   (t, ts) = cps_app_ts xvs ∧
   inner = cps_transform_letinit
     ((x,Var (Short t))::ZIP (MAP FST xvs, MAP (Var o Short) ts))
     bs e (Var (Short "k")) ∧
-  LIST_REL (ml_v_vals refs) (MAP SND xvs) mlvs ∧
+  LIST_REL ml_v_vals (MAP SND xvs) mlvs ∧
   LIST_REL (λ x mlv . nsLookup env.v (Short x) = SOME mlv) ts mlvs ∧
   scheme_env env ∧
-  env_rel refs se env
+  env_rel se env
   ⇒
-  cont_rel refs ((se, LetinitK xvs x bs e) :: ks)
+  cont_rel ((se, LetinitK xvs x bs e) :: ks)
     (Closure env t $ inner)
 End
 
@@ -421,326 +286,49 @@ Theorem val_cont_rels_ind[allow_rebind] = SRULE [] $ val_cont_rels_ind;
 Theorem ml_v_vals_cases = SRULE [] $ cj 1 val_cont_rels_cases;
 Theorem cont_rel_cases = cj 2 val_cont_rels_cases;
 
-Theorem val_cont_rel_mono:
-  ! refs mlv' .
-    (! v mlv . ml_v_vals refs v mlv ==> ml_v_vals (refs ++ [Refv mlv']) v mlv) /\
-    (! ks kv . cont_rel refs ks kv ==> cont_rel (refs ++ [Refv mlv']) ks kv)
-Proof
-  rpt gen_tac
-  >> ho_match_mp_tac val_cont_rels_ind
-  >> rpt strip_tac
-  >> simp[Once ml_v_vals_cases, env_rel_alloc]
-  >- (
-    irule_at (Pos hd) EQ_REFL >> gvs[SF ETA_ss]
-  )
-  >- (
-    simp[pairs_loc_alloc_diff]
-    >> simp[GSYM pairs_loc_alloc_diff]
-  )
-  >> simp[Once cont_rel_cases, env_rel_alloc]
-  >> irule_at (Pos hd) EQ_REFL
-  >> first_assum $ irule_at (Pos last)
-  >> gvs[SF ETA_ss]
-QED
-
-Theorem ml_v_vals_mono = SRULE [PULL_FORALL, AND_IMP_INTRO] $
-  cj 1 val_cont_rel_mono;
-Theorem cont_rel_mono = SRULE [PULL_FORALL, AND_IMP_INTRO] $
-  cj 2 val_cont_rel_mono;
-
-Theorem val_cont_rel_LUPDATE_same:
-  ! refs l mlv'1 mlv'2 .
-    EL l refs = Refv mlv'1
-    ==>
-    (! v mlv . ml_v_vals refs v mlv ==> ml_v_vals (LUPDATE (Refv mlv'2) l refs) v mlv) /\
-    (! ks kv . cont_rel refs ks kv ==> cont_rel (LUPDATE (Refv mlv'2) l refs) ks kv)
-Proof
-  rpt gen_tac >> strip_tac
-  >> ho_match_mp_tac val_cont_rels_ind
-  >> rpt strip_tac
-  >> simp[Once ml_v_vals_cases] >- simp[env_rel_LUPDATE_same]
-  >- (
-    irule_at (Pos hd) EQ_REFL >> gvs[SF ETA_ss]
-  )
-  >- (
-    simp[pairs_loc_LUPDATE_diff]
-    >> simp[GSYM pairs_loc_LUPDATE_diff]
-  )
-  >> simp[Once cont_rel_cases, env_rel_LUPDATE_same]
-  >> irule_at (Pos hd) EQ_REFL
-  >> first_assum $ irule_at (Pos last)
-  >> gvs[SF ETA_ss]
-QED
-
-Theorem ml_v_vals_LUPDATE_same = SRULE [PULL_FORALL, AND_IMP_INTRO] $
-  cj 1 val_cont_rel_LUPDATE_same;
-Theorem cont_rel_LUPDATE_same = SRULE [PULL_FORALL, AND_IMP_INTRO] $
-  cj 2 val_cont_rel_LUPDATE_same;
-
 val (store_entry_rel_rules,store_entry_rel_ind,store_entry_rel_cases) =
 (fn (x,y,z) => (SRULE [] x,SRULE [] y, SRULE [] z)) $ Hol_reln ‘
-  (ml_v_vals refs v mlv
+  store_entry_rel (Mut NONE) (Refv (Conv (SOME (scheme_typestamp "None")) [])) ∧
+  (ml_v_vals v mlv
   ⇒
-  store_entry_rel refs (SOME v) (Refv (Conv (SOME (scheme_typestamp "Some")) [mlv]))) ∧
-  store_entry_rel refs NONE (Refv (Conv (SOME (scheme_typestamp "None")) []))
+  store_entry_rel (Mut (SOME v)) (Refv (Conv (SOME (scheme_typestamp "Some")) [mlv]))) ∧
+  (ml_v_vals v1 mlv1 ∧
+  ml_v_vals v2 mlv2
+  ⇒
+  store_entry_rel (Pair (v1, v2)) (Varray [mlv1; mlv2]))
 ’;
-
-Inductive pair_rel:
-  ml_v_vals refs v mlv ∧
-  ml_v_vals refs v' mlv'
-  ⇒
-  pair_rel refs (v, v') (Varray [mlv; mlv'])
-End
-
-Inductive muts_rel:
-[~empty:]
-  muts_rel refs' [] []
-[~mut:]
-  store_entry_rel refs' mut ref ∧
-  muts_rel refs' muts refs
-  ⇒
-  muts_rel refs' (mut::muts) (ref::refs)
-[~pair:]
-  muts_rel refs' muts refs
-  ⇒
-  muts_rel refs' muts (Varray vs::refs)
-End
-
-Inductive pairs_rel:
-[~empty:]
-  pairs_rel refs' [] []
-[~pair:]
-  pair_rel refs' pair ref ∧
-  pairs_rel refs' pairs refs
-  ⇒
-  pairs_rel refs' (pair::pairs) (ref::refs)
-[~mut:]
-  pairs_rel refs' pairs refs
-  ⇒
-  pairs_rel refs' pairs (Refv v::refs)
-End
-
-Definition store_rel_def[simp]:
-  store_rel st refs <=> muts_rel refs st.muts refs ∧ pairs_rel refs st.pairs refs
-End
-
-Theorem muts_rel_FILTER:
-  ! refs' muts refs .
-    muts_rel refs' muts refs
-    ==>
-    LIST_REL (store_entry_rel refs') muts $
-      FILTER (\ref. case ref of | Refv _ => T | _ => F) refs
-Proof
-  gen_tac >> ho_match_mp_tac muts_rel_ind
-  >> simp[]
-  >> rpt strip_tac
-  >> CASE_TAC
-  >> gvs[Once store_entry_rel_cases]
-  >> simp[Once store_entry_rel_cases]
-QED
-
-Theorem muts_rel_LUPDATE_same:
-  ! refs' muts refs .
-    muts_rel refs' muts refs
-    ==>
-    ! mut ref l .
-      store_entry_rel refs' mut ref
-      ==>
-      muts_rel refs' muts refs /\
-      muts_rel refs' (LUPDATE mut l muts) (LUPDATE ref (muts_loc 0 refs l) refs)
-Proof
-  gen_tac
-  >> ho_match_mp_tac muts_rel_ind
-  >> simp[LUPDATE_def]
-  >> simp[Once muts_rel_cases]
-  >> rpt strip_tac >- (
-    first_x_assum $ drule >> strip_tac
-    >> simp[Once muts_rel_cases]
-  )
-  >- (
-    gvs[Once store_entry_rel_cases]
-    >> Cases_on `l`
-    >> gvs[LUPDATE_def, muts_loc_def]
-    >> first_x_assum $ drule >> strip_tac
-    >> simp[Once muts_rel_cases]
-    >> simp[store_entry_rel_cases]
-  )
-  >- (
-    irule muts_rel_pair
-    >> last_x_assum drule >> strip_tac
-    >> simp[]
-  )
-  >> simp[muts_loc_def, LUPDATE_def, Once muts_rel_cases]
-QED
-
-Theorem muts_rel_LUPDATE_same[allow_rebind] = cj 2 muts_rel_LUPDATE_same;
-
-Theorem muts_rel_mono:
-  ! (refs'1:'a store_v list) (refs'2:'a store_v list) .
-    (! mut ref . store_entry_rel refs'1 mut ref ==> store_entry_rel refs'2 mut ref)
-    ==>
-    ! muts refs .
-      muts_rel refs'1 muts refs ==> muts_rel refs'2 muts refs
-Proof
-  rpt gen_tac >> strip_tac
-  >> ho_match_mp_tac muts_rel_ind
-  >> rpt strip_tac
-  >> gvs[store_entry_rel_cases]
-  >> simp[Once muts_rel_cases]
-  >> simp[store_entry_rel_cases]
-QED
-
-Theorem muts_rel_loc:
-  ! refs' muts refs l .
-    l < LENGTH muts /\ muts_rel refs' muts refs 
-    ==>
-    muts_loc 0 refs l < LENGTH refs /\
-    store_entry_rel refs' (EL l muts) (EL (muts_loc 0 refs l) refs)
-Proof
-  rpt strip_tac
-  >> dxrule_then assume_tac muts_rel_FILTER
-  >> gvs[LIST_REL_EL_EQN, muts_loc_FILTER]
-QED
-
-Theorem muts_rel_loc_alloc:
-  ! mlv muts refs .
-    muts_rel refs muts refs
-    ==>
-    muts_loc 0 refs (LENGTH muts) = LENGTH refs
-Proof
-  rpt strip_tac
-  >> dxrule_then assume_tac muts_rel_FILTER
-  >> dxrule_then assume_tac LIST_REL_LENGTH
-  >> simp[muts_loc_FILTER]
-QED
-
-Theorem pairs_rel_FILTER:
-  ! refs' pairs refs .
-    pairs_rel refs' pairs refs
-    ==>
-    LIST_REL (pair_rel refs') pairs $
-      FILTER (\ref. case ref of | Varray _ => T | _ => F) refs
-Proof
-  gen_tac >> ho_match_mp_tac pairs_rel_ind
-  >> simp[]
-  >> rpt strip_tac
-  >> CASE_TAC
-  >> gvs[Once pair_rel_cases]
-  >> simp[Once pair_rel_cases]
-QED
-
-Theorem pairs_rel_LUPDATE_diff:
-  ! refs' pairs refs .
-    pairs_rel refs' pairs refs
-    ==>
-    ! mut ref l .
-      store_entry_rel refs' mut ref
-      ==>
-      pairs_rel refs' pairs refs /\
-      pairs_rel refs' pairs (LUPDATE ref (muts_loc 0 refs l) refs)
-Proof
-  gen_tac
-  >> ho_match_mp_tac pairs_rel_ind
-  >> simp[LUPDATE_def]
-  >> simp[Once pairs_rel_cases]
-  >> rpt strip_tac
-  >> first_x_assum $ drule_then $ mp_tac o SRULE [Once $ GSYM PULL_FORALL]
-  >> strip_tac
-  >~ [`muts_loc 0 (Refv _::_) _`]
-  >- (
-    Cases_on `l`
-    >> simp[LUPDATE_def, muts_loc_def]
-    >> gvs[Once store_entry_rel_cases]
-    >> simp[Once pairs_rel_cases]
-    >> simp[Once pairs_rel_cases]
-  )
-  >> gvs[Once pair_rel_cases]
-  >> simp[LUPDATE_def, muts_loc_def]
-  >> simp[Once pairs_rel_cases]
-  >> simp[Once pair_rel_cases]
-QED
-
-Theorem pairs_rel_LUPDATE_diff[allow_rebind] = cj 2 pairs_rel_LUPDATE_diff;
-
-Theorem pairs_rel_mono:
-  ! (refs'1:'a store_v list) (refs'2:'a store_v list) .
-    (! pair ref . pair_rel refs'1 pair ref ==> pair_rel refs'2 pair ref)
-    ==>
-    ! pairs refs .
-      pairs_rel refs'1 pairs refs ==> pairs_rel refs'2 pairs refs
-Proof
-  rpt gen_tac >> strip_tac
-  >> ho_match_mp_tac pairs_rel_ind
-  >> rpt strip_tac
-  >> gvs[pair_rel_cases]
-  >> simp[Once pairs_rel_cases]
-  >> simp[pair_rel_cases]
-QED
-
-Theorem pairs_rel_loc:
-  ! refs' pairs refs l .
-    l < LENGTH pairs /\ pairs_rel refs' pairs refs 
-    ==>
-    pairs_loc 0 refs l < LENGTH refs /\
-    pair_rel refs' (EL l pairs) (EL (pairs_loc 0 refs l) refs)
-Proof
-  rpt strip_tac
-  >> dxrule_then assume_tac pairs_rel_FILTER
-  >> gvs[LIST_REL_EL_EQN, pairs_loc_FILTER]
-QED
-
-(*
-Inductive e_ce_rel:
-[~Val:]
-  ml_v_vals v mlv ∧
-  nsLookup env.v (Short valv) = SOME (mlv) ∧
-  nsLookup env.v (Short var) = SOME kv ∧
-  valv ≠ var
-  ⇒
-  e_ce_rel (Val v) var env kv $ App Opapp [Var (Short var); Var (Short valv)]
-[~Exp:]
-  ce = cps_transform e ∧
-  nsLookup env.v (Short var) = SOME kv ∧
-  scheme_env env
-  ⇒
-  e_ce_rel (Exp e) var env kv $ App Opapp [ce; Var (Short var)]
-[~Exception:]
-  e_ce_rel (Exception s) var env kv $
-    Con (SOME $ Short "Ex") [Lit $ StrLit $ explode s]
-End
-*)
 
 Inductive cps_rel:
 [~Val:]
-  ml_v_vals refs v mlv ∧
+  ml_v_vals v mlv ∧
   nsLookup env.v (Short t) = SOME (mlv) ∧
   nsLookup env.v (Short k) = SOME kv ∧
   t ≠ k
   ⇒
-  cps_rel refs (Val v) k env kv $ App Opapp [Var (Short k); Var (Short t)]
+  cps_rel (Val v) k env kv $ App Opapp [Var (Short k); Var (Short t)]
 [~Exp:]
   ce = cps_transform e ∧
   nsLookup env.v (Short k) = SOME kv ∧
   scheme_env env ∧
-  env_rel refs senv env
+  env_rel senv env
   ⇒
-  cps_rel refs (Exp senv e) var env kv $ App Opapp [ce; Var (Short k)]
+  cps_rel (Exp senv e) var env kv $ App Opapp [ce; Var (Short k)]
 [~Exception:]
-  cps_rel refs (Exception s) var env kv $
+  cps_rel (Exception s) var env kv $
     Con (SOME $ Short "Ex") [Lit $ StrLit $ explode s]
 End
 
 Theorem env_rel_FEMPTY[simp]:
-  ∀ refs env . env_rel refs FEMPTY env
+  ∀ env . env_rel FEMPTY env
 Proof
   simp[env_rel_cases, FEVERY_FEMPTY]
 QED
 
 Theorem env_rel_non_var[simp]:
-  ! refs se env envv var v .
+  ! se env envv var v .
     (! x . var <> "var" ++ x)
     ==>
-    env_rel refs se (env with v := nsBind var v envv) = env_rel refs se (env with v := envv)
+    env_rel se (env with v := nsBind var v envv) = env_rel se (env with v := envv)
 Proof
   simp[env_rel_cases]
 QED
@@ -761,8 +349,8 @@ Theorem compile_in_rel:
     scheme_env env
     ⇒
     ∃ st' env' var mle ks kv .
-      cps_rel st.refs (Exp FEMPTY p) var env' kv mle ∧
-      cont_rel st.refs ks kv ∧
+      cps_rel (Exp FEMPTY p) var env' kv mle ∧
+      cont_rel ks kv ∧
       evaluate st env [compile_scheme_prog p] = evaluate st' env' [mle]
 Proof
   simp[Once cps_rel_cases, compile_scheme_prog_def]
@@ -862,29 +450,6 @@ Proof
   >> gvs[scheme_env_def]
 QED
 
-Theorem map_reverse(*[simp]*):
-  ∀ xs f . MAP f (REVERSE xs) = REVERSE (MAP f xs)
-Proof
-  Induct >> simp[]
-QED
-
-Theorem LIST_REL_SNOC_ind:
-  ∀R LIST_REL'.
-    LIST_REL' [] [] ∧
-    (∀h1 h2 t1 t2.
-      R h1 h2 ∧ LIST_REL' t1 t2 ⇒ LIST_REL' (SNOC h1 t1) (SNOC h2 t2)) ⇒
-    ∀a0 a1. LIST_REL R a0 a1 ⇒ LIST_REL' a0 a1
-Proof
-  strip_tac >> strip_tac >> strip_tac
-  >> Induct_on ‘a0’ using SNOC_INDUCT
-  >> Induct_on ‘a1’ using SNOC_INDUCT
-  >- simp[]
-  >- simp[EVERY2_LENGTH]
-  >- simp[EVERY2_LENGTH]
-  >> pop_assum kall_tac
-  >> simp[LIST_REL_SNOC]
-QED
-
 Definition eval_eq_def:
   eval_eq st mlenv mle st' mlenv' mle' ck = ∀ start.
     evaluate (st with clock := ck + start) mlenv [mle]
@@ -921,668 +486,107 @@ Definition ex_eval_def:
   ex_eval st env s = evaluate st env [Con (SOME $ Short "Ex") [Lit $ StrLit s]]
 End
 
-Theorem preservation_of_sadd_body:
-  ∀ vs mlvs .
-    LIST_REL ml_v_vals vs mlvs
-    ⇒
-  ∀ store st env n k kv .
-    cont_rel k kv ∧
-    LIST_REL store_entry_rel store st.refs ∧
-    nsLookup env.v (Short "ts") = SOME (vcons_list mlvs) ∧
-    nsLookup env.v (Short "n") = SOME (Litv (IntLit n)) ∧
-    nsLookup env.v (Short "k") = SOME kv ∧
-    nsLookup env.v (Short "sadd") = nsLookup scheme_env2.v (Short "sadd") ∧
-    env.c = scheme_env1.c
-    ⇒
-    ∃ck st' mlenv' var' kv' mle'.
-      (∀ start . evaluate (st with clock := ck + start) env
-        [Mat (Var (Short "ts"))
-           [(Pcon (SOME (Short "[]")) [],
-             Let (SOME "t") (Con (SOME (Short "SNum")) [Var (Short "n")])
-               (App Opapp [Var (Short "k"); Var (Short "t")]));
-            (Pcon (SOME (Short "::")) [Pvar "t"; Pvar "ts'"],
-             Mat (Var (Short "t"))
-               [(Pcon (SOME (Short "SNum")) [Pvar "tn"],
-                 App Opapp
-                   [App Opapp
-                      [App Opapp [Var (Short "sadd"); Var (Short "k")];
-                       App (Opn Plus) [Var (Short "n"); Var (Short "tn")]];
-                    Var (Short "ts'")]);
-                (Pany,
-                 Con (SOME (Short "Ex"))
-                   [Lit (StrLit "Arith-op applied to non-number")])])]] =
-      evaluate (st' with clock := start) mlenv' [mle']) ∧
-      cont_rel k kv' ∧
-      e_ce_rel (sadd vs n) var' mlenv' kv' mle' ∧
-      env_rel FEMPTY mlenv' ∧
-      LIST_REL store_entry_rel store st'.refs ∧
-      st.ffi = st'.ffi
+Theorem state_ffi_trivial[simp]:
+  ! st:'ffi state . st with ffi := st.ffi = st
 Proof
-  ho_match_mp_tac LIST_REL_ind
-  >> simp[vcons_list_def, sadd_def]
-  >> rpt strip_tac >- (
-    simp[Ntimes evaluate_def 2]
-    >> simp[can_pmatch_all_def, pmatch_def, nsLookup_def,
-      same_type_def, same_ctor_def, evaluate_match_def,
-      pat_bindings_def]
-    >> simp[Ntimes evaluate_def 3, do_con_check_def, build_conv_def,
-      nsOptBind_def]
-    >> simp[GSYM eval_eq_def]
-    >> irule_at (Pos hd) eval_eq_trivial
-    >> last_assum $ irule_at (Pos hd)
-    >> simp[Once e_ce_rel_cases, sadd_def, Once ml_v_vals_cases,
-      env_rel_cases, FEVERY_FEMPTY]
-  )
-  >> gvs[Once ml_v_vals_cases]
-  >> gvs[vcons_list_def]
-  >~ [‘SNum m’] >- (
-    simp[sadd_def]
-    >> simp[evaluate_def, do_opapp_def, do_app_def,
-      opn_lookup_def, can_pmatch_all_def, pmatch_def, nsLookup_def,
-      same_type_def, same_ctor_def, evaluate_match_def,
-      pat_bindings_def, do_con_check_def, build_conv_def, dec_clock_def]
-    >> simp[Ntimes find_recfun_def 2, Ntimes build_rec_env_def 2]
-    >> qrefine ‘ck+3’
-    >> simp[Ntimes evaluate_def 2]
-    >> ‘st.ffi = (st with <|refs := st.refs; ffi := st.ffi|>).ffi’ by simp[]
-    >> first_assum $ once_asm_rewrite_tac o single
-    >> pop_assum $ simp_tac pure_ss o single o Once o GSYM
-    >> last_x_assum irule
-    >> simp[]
-    >> simp[Once INT_ADD_COMM]
-  )
-  >> simp[Ntimes evaluate_def 10, do_opapp_def, do_app_def,
-    opn_lookup_def, can_pmatch_all_def, pmatch_def, nsLookup_def,
-    same_type_def, same_ctor_def, evaluate_match_def,
-    pat_bindings_def, do_con_check_def, build_conv_def, dec_clock_def]
-  >> simp[Ntimes find_recfun_def 2, Ntimes build_rec_env_def 2]
-  >> simp[sadd_def, Once e_ce_rel_cases]
-  >> simp[GSYM eval_eq_def]
-  >> irule_at (Pos hd) eval_eq_trivial
-  >> qpat_assum ‘cont_rel _ _’ $ irule_at (Pos hd)
-  >> simp[env_rel_cases, FEVERY_FEMPTY]
+  simp[state_component_equality]
 QED
 
-Theorem preservation_of_smul_body:
-  ∀ vs mlvs .
-    LIST_REL ml_v_vals vs mlvs
-    ⇒
-  ∀ store st env n k kv .
-    cont_rel k kv ∧
-    LIST_REL store_entry_rel store st.refs ∧
-    nsLookup env.v (Short "ts") = SOME (vcons_list mlvs) ∧
-    nsLookup env.v (Short "n") = SOME (Litv (IntLit n)) ∧
-    nsLookup env.v (Short "k") = SOME kv ∧
-    nsLookup env.v (Short "smul") = nsLookup scheme_env3.v (Short "smul") ∧
-    env.c = scheme_env1.c
-    ⇒
-    ∃ck st' mlenv' var' kv' mle'.
-      (∀ start . evaluate (st with clock := ck + start) env
-        [Mat (Var (Short "ts"))
-           [(Pcon (SOME (Short "[]")) [],
-             Let (SOME "t") (Con (SOME (Short "SNum")) [Var (Short "n")])
-               (App Opapp [Var (Short "k"); Var (Short "t")]));
-            (Pcon (SOME (Short "::")) [Pvar "t"; Pvar "ts'"],
-             Mat (Var (Short "t"))
-               [(Pcon (SOME (Short "SNum")) [Pvar "tn"],
-                 App Opapp
-                   [App Opapp
-                      [App Opapp [Var (Short "smul"); Var (Short "k")];
-                       App (Opn Times) [Var (Short "n"); Var (Short "tn")]];
-                    Var (Short "ts'")]);
-                (Pany,
-                 Con (SOME (Short "Ex"))
-                   [Lit (StrLit "Arith-op applied to non-number")])])]] =
-      evaluate (st' with clock := start) mlenv' [mle']) ∧
-      cont_rel k kv' ∧
-      e_ce_rel (smul vs n) var' mlenv' kv' mle' ∧
-      env_rel FEMPTY mlenv' ∧
-      LIST_REL store_entry_rel store st'.refs ∧
-      st.ffi = st'.ffi
+Theorem state_refs_trivial[simp]:
+  ! st:'ffi state . st with refs := st.refs = st
 Proof
-  ho_match_mp_tac LIST_REL_ind
-  >> simp[vcons_list_def, smul_def]
-  >> rpt strip_tac >- (
-    simp[Ntimes evaluate_def 2]
-    >> simp[can_pmatch_all_def, pmatch_def, nsLookup_def,
-      same_type_def, same_ctor_def, evaluate_match_def,
-      pat_bindings_def]
-    >> simp[Ntimes evaluate_def 3, do_con_check_def, build_conv_def,
-      nsOptBind_def]
-    >> simp[GSYM eval_eq_def]
-    >> irule_at (Pos hd) eval_eq_trivial
-    >> last_assum $ irule_at (Pos hd)
-    >> simp[Once e_ce_rel_cases, smul_def, Once ml_v_vals_cases,
-      env_rel_cases, FEVERY_FEMPTY]
-  )
-  >> gvs[Once ml_v_vals_cases]
-  >> gvs[vcons_list_def]
-  >~ [‘SNum m’] >- (
-    simp[smul_def]
-    >> simp[evaluate_def, do_opapp_def, do_app_def,
-      opn_lookup_def, can_pmatch_all_def, pmatch_def, nsLookup_def,
-      same_type_def, same_ctor_def, evaluate_match_def,
-      pat_bindings_def, do_con_check_def, build_conv_def, dec_clock_def]
-    >> simp[Ntimes find_recfun_def 2, Ntimes build_rec_env_def 2]
-    >> qrefine ‘ck+3’
-    >> simp[Ntimes evaluate_def 2]
-    >> ‘st.ffi = (st with <|refs := st.refs; ffi := st.ffi|>).ffi’ by simp[]
-    >> first_assum $ once_asm_rewrite_tac o single
-    >> pop_assum $ simp_tac pure_ss o single o Once o GSYM
-    >> last_x_assum irule
-    >> simp[]
-    >> simp[scheme_env2_def, Once INT_MUL_COMM]
-  )
-  >> simp[Ntimes evaluate_def 10, do_opapp_def, do_app_def,
-    opn_lookup_def, can_pmatch_all_def, pmatch_def, nsLookup_def,
-    same_type_def, same_ctor_def, evaluate_match_def,
-    pat_bindings_def, do_con_check_def, build_conv_def, dec_clock_def]
-  >> simp[Ntimes find_recfun_def 2, Ntimes build_rec_env_def 2]
-  >> simp[smul_def, Once e_ce_rel_cases]
-  >> simp[GSYM eval_eq_def]
-  >> irule_at (Pos hd) eval_eq_trivial
-  >> qpat_assum ‘cont_rel _ _’ $ irule_at (Pos hd)
-  >> simp[env_rel_cases, FEVERY_FEMPTY]
+  simp[state_component_equality]
 QED
 
-Theorem preservation_of_sminus_body:
-  ∀ vs mlvs .
-    LIST_REL ml_v_vals vs mlvs
-    ⇒
-  ∀ store (st:'ffi state) env n k kv .
-    cont_rel k kv ∧
-    LIST_REL store_entry_rel store st.refs ∧
-    nsLookup env.v (Short "ts") = SOME (vcons_list mlvs) ∧
-    nsLookup env.v (Short "k") = SOME kv ∧
-    nsLookup env.v (Short "sadd") = nsLookup scheme_env3.v (Short "sadd") ∧
-    env.c = scheme_env1.c
-    ⇒
-    ∃ck st' mlenv' var' kv' mle'.
-      (∀ start . evaluate (st with clock := ck + start) env
-        [Mat (Var (Short "ts"))
-           [(Pcon (SOME (Short "[]")) [],
-             Con (SOME (Short "Ex")) [Lit (StrLit "Arity mismatch")]);
-            (Pcon (SOME (Short "::")) [Pvar "t"; Pvar "ts'"],
-             Mat (Var (Short "t"))
-               [(Pcon (SOME (Short "SNum")) [Pvar "n"],
-                  Mat (Var (Short "ts'")) [
-                    (Pcon (SOME $ Short "[]") [],
-                      Let (SOME "t") (Con (SOME $ Short "SNum") [
-                          App (Opn Minus) [Lit $ IntLit 0; Var (Short "n")]]) $
-                        App Opapp [Var (Short "k"); Var (Short "t")]);
-                    (Pany, App Opapp [App Opapp [App Opapp [Var (Short "sadd");
-                      Fun "t" $ Mat (Var (Short "t")) [
-                        (Pcon (SOME $ Short "SNum") [Pvar "m"],
-                          Let (SOME "t") (Con (SOME $ Short "SNum") [
-                              App (Opn Minus) [Var (Short "n"); Var (Short "m")]]) $
-                            App Opapp [Var (Short "k"); Var (Short "t")]);
-                        (Pany,
-                          App Opapp [Var (Short "k"); Var (Short "t")])
-                      ]];
-                      Lit $ IntLit 0]; Var (Short "ts'")])]);
-                (Pany,
-                 Con (SOME (Short "Ex"))
-                   [Lit (StrLit "Arith-op applied to non-number")])])]] =
-      evaluate (st' with clock := start) mlenv' [mle']) ∧
-      cont_rel k kv' ∧
-      e_ce_rel (sminus vs) var' mlenv' kv' mle' ∧
-      env_rel FEMPTY mlenv' ∧
-      LIST_REL store_entry_rel store st'.refs ∧
-      st.ffi = st'.ffi
-Proof
-  Cases_on ‘vs’ >- (
-    simp[vcons_list_def]
-    >> rpt strip_tac
-    >> simp[Ntimes evaluate_def 3]
-    >> simp[can_pmatch_all_def, pmatch_def, nsLookup_def,
-      same_type_def, same_ctor_def, evaluate_match_def,
-      pat_bindings_def]
-    >> simp[GSYM eval_eq_def]
-    >> irule_at (Pos hd) eval_eq_trivial
-    >> last_assum $ irule_at (Pos hd)
-    >> simp[sminus_def]
-    >> simp[Once e_ce_rel_cases, env_rel_cases, FEVERY_FEMPTY]
-  )
-  >> Cases_on ‘mlvs’
-  >> simp[vcons_list_def]
-  >> strip_tac
-  >> gvs[Once ml_v_vals_cases]
-  >~ [‘SNum i’] >- (
-    simp[Ntimes evaluate_def 3]
-    >> simp[can_pmatch_all_def, pmatch_def, nsLookup_def,
-      same_type_def, same_ctor_def, evaluate_match_def,
-      pat_bindings_def]
-    >> rpt strip_tac
-    >> simp[Ntimes evaluate_def 3]
-    >> simp[can_pmatch_all_def, pmatch_def, nsLookup_def,
-      same_type_def, same_ctor_def, evaluate_match_def,
-      pat_bindings_def]
-    >> simp[Ntimes find_recfun_def 2, Ntimes build_rec_env_def 2]
-    >> Cases_on ‘t=[]’ >- (
-      gvs[vcons_list_def]
-      >> simp[Ntimes evaluate_def 3]
-      >> simp[can_pmatch_all_def, pmatch_def, nsLookup_def,
-        same_type_def, same_ctor_def, evaluate_match_def,
-        pat_bindings_def]
-      >> simp[Ntimes evaluate_def 6, do_app_def, do_con_check_def,
-        build_conv_def, nsOptBind_def, opn_lookup_def]
-      >> simp[GSYM eval_eq_def]
-      >> irule_at (Pos hd) eval_eq_trivial
-      >> simp[sminus_def, Once e_ce_rel_cases, Once ml_v_vals_cases,
-        env_rel_cases, FEVERY_FEMPTY]
-    )
-    >> qrefine ‘ck+3’
-    >> ‘∃ t' ts' . t'::ts'=t’ by (Cases_on ‘t’ >> gvs[])
-    >> simp[sminus_def]
-    >> first_assum $ simp_tac bool_ss o single o  GSYM
-    >> simp[Ntimes evaluate_def 3]
-    >> ‘∃ y ys . y::ys = t'’ by gvs[]
-    >> pop_assum $ simp_tac bool_ss o single o (fn x => Ntimes x 2) o GSYM
-    >> simp[vcons_list_def]
-    >> simp[can_pmatch_all_def, pmatch_def, nsLookup_def,
-      same_type_def, same_ctor_def, evaluate_match_def,
-      pat_bindings_def]
-    >> pop_assum kall_tac
-    >> pop_assum kall_tac
-    >> simp[Ntimes evaluate_def 3]
-    >> simp[can_pmatch_all_def, pmatch_def, nsLookup_def,
-      same_type_def, same_ctor_def, evaluate_match_def,
-      pat_bindings_def]
-    >> simp[Ntimes evaluate_def 7, do_opapp_def]
-    >> simp[Ntimes find_recfun_def 2, Ntimes build_rec_env_def 2]
-    >> simp[Ntimes evaluate_def 2, dec_clock_def]
-    >> simp[sminus_def]
-    >> ‘∃ n . 0i = n’ by simp[]
-    >> pop_assum mp_tac >> strip_tac
-    >> pop_assum $ simp o single
-    >> ‘∃ kenv . (env with
-                           v :=
-                             nsBind "n" (Litv (IntLit i))
-                               (nsBind "ts'" (vcons_list t')
-                                  (nsBind "t"
-                                     (Conv (SOME (TypeStamp "SNum" 4))
-                                        [Litv (IntLit i)]) env.v)))
-                  = kenv’ by simp[]
-    >> pop_assum mp_tac >> strip_tac
-    >> ‘nsLookup kenv.v (Short "n") = SOME (Litv (IntLit i))’ by gvs[]
-    >> ‘nsLookup kenv.v (Short "k") = SOME kv’ by gvs[]
-    >> ‘kenv.c = scheme_env1.c’ by gvs[]
-    >> qpat_x_assum ‘_ = kenv’ $ simp o single
-    >> rpt $ qpat_x_assum ‘nsLookup env.v _ = _’ kall_tac
-    >> rpt $ pop_assum mp_tac
-    >> strip_tac
-    >> qid_spec_tac ‘i''’
-    >> qid_spec_tac ‘n’
-    >> qid_spec_tac ‘st’
-    >> pop_assum mp_tac
-    >> qid_spec_tac ‘t'’
-    >> qid_spec_tac ‘t’
-    >> ho_match_mp_tac LIST_REL_ind
-    >> rpt strip_tac >- (
-      simp[vcons_list_def, sadd_def]
-      >> simp[Ntimes evaluate_def 3]
-      >> simp[can_pmatch_all_def, pmatch_def, nsLookup_def,
-        same_type_def, same_ctor_def, evaluate_match_def,
-        pat_bindings_def]
-      >> simp[Ntimes evaluate_def 7, do_opapp_def, do_con_check_def,
-        build_conv_def, nsOptBind_def]
-      >> qrefine ‘ck+1’
-      >> simp[Ntimes evaluate_def 3, dec_clock_def]
-      >> simp[can_pmatch_all_def, pmatch_def, nsLookup_def,
-        same_type_def, same_ctor_def, evaluate_match_def,
-        pat_bindings_def]
-      >> simp[Ntimes evaluate_def 6, do_app_def, do_con_check_def,
-        build_conv_def, nsOptBind_def, opn_lookup_def]
-      >> simp[GSYM eval_eq_def]
-      >> irule_at (Pos hd) eval_eq_trivial
-      >> simp[env_rel_cases, FEVERY_FEMPTY]
-      >> qpat_assum ‘cont_rel _ _’ $ irule_at (Pos hd)
-      >> simp[Once e_ce_rel_cases, Once ml_v_vals_cases]
-    )
-    >> gvs[Once ml_v_vals_cases]
-    >~ [‘SNum m’] >- (
-      simp[sadd_def, vcons_list_def]
-      >> simp[evaluate_def, do_opapp_def, do_app_def,
-        opn_lookup_def, can_pmatch_all_def, pmatch_def, nsLookup_def,
-        same_type_def, same_ctor_def, evaluate_match_def,
-        pat_bindings_def, do_con_check_def, build_conv_def, dec_clock_def]
-      >> simp[Ntimes find_recfun_def 2, Ntimes build_rec_env_def 2]
-      >> qrefine ‘ck+3’
-      >> simp[Ntimes evaluate_def 2]
-      >> simp[Once INT_ADD_COMM]
-      >> ‘st.ffi = (st with <|refs := st.refs; ffi := st.ffi|>).ffi’ by simp[]
-      >> first_assum $ once_asm_rewrite_tac o single
-      >> pop_assum $ simp_tac pure_ss o single o Once o GSYM
-      >> last_x_assum irule
-      >> simp[]
-    )
-    >> simp[sadd_def, vcons_list_def]
-    >> simp[Ntimes evaluate_def 3]
-    >> simp[can_pmatch_all_def, pmatch_def, nsLookup_def,
-      same_type_def, same_ctor_def, evaluate_match_def,
-      pat_bindings_def]
-    >> simp[Ntimes evaluate_def 3]
-    >> simp[can_pmatch_all_def, pmatch_def, nsLookup_def,
-      same_type_def, same_ctor_def, evaluate_match_def,
-      pat_bindings_def]
-    >> simp[GSYM eval_eq_def]
-    >> irule_at (Pos hd) eval_eq_trivial
-    >> simp[env_rel_cases, FEVERY_FEMPTY]
-    >> qpat_assum ‘cont_rel _ _’ $ irule_at (Pos hd)
-    >> simp[Once e_ce_rel_cases]
-  )
-  >> simp[sminus_def]
-  >> rpt strip_tac
-  >> simp[Ntimes evaluate_def 3]
-  >> simp[can_pmatch_all_def, pmatch_def, nsLookup_def,
-    same_type_def, same_ctor_def, evaluate_match_def,
-    pat_bindings_def]
-  >> simp[Ntimes evaluate_def 3]
-  >> simp[can_pmatch_all_def, pmatch_def, nsLookup_def,
-    same_type_def, same_ctor_def, evaluate_match_def,
-    pat_bindings_def]
-  >> simp[GSYM eval_eq_def]
-  >> irule_at (Pos hd) eval_eq_trivial
-  >> simp[env_rel_cases, FEVERY_FEMPTY]
-  >> qpat_assum ‘cont_rel _ _’ $ irule_at (Pos hd)
-  >> simp[Once e_ce_rel_cases]
-QED
+Definition letpreinit_mlenv_def:
+  letpreinit_mlenv mlenv xs l
+  =
+  (mlenv with v := nsAppend (Bind (REVERSE $ MAP (\ p. ("var" ++ (explode $ FST p), Loc T $ l + SND p)) $ ZIP (xs, GENLIST I $ LENGTH xs)) []) mlenv.v)
+End
 
-Theorem preservation_of_proc:
-∀ (st:'ffi state) inner n n' m m' env env' mlenv var kv n xs xp e e' ce k args vs mlvs store store' .
-  valid_val store (Proc env xs xp e) ∧
-  LIST_REL ml_v_vals vs mlvs ∧
-  EVERY (valid_val store) vs ∧
-  valid_cont store k ∧
-  cont_rel k kv ∧
-  ce = cps_transform e ∧
-  inner = proc_ml xs xp "k" ce ∧
-  (store', env',e') = parameterize store env xs xp e vs ∧
-  EVERY (OPTION_ALL (valid_val store)) store ∧
-  nsLookup mlenv.v (Short "k") = SOME kv ∧
-  nsLookup mlenv.v (Short "ts") = SOME (vcons_list mlvs) ∧
-  env_rel env mlenv ∧
-  scheme_env mlenv ∧
-  can_lookup env store ∧
-  LIST_REL store_entry_rel store st.refs
-  ⇒
-  ∃ck st' mlenv' var' kv' mle'.
-    (∀ start . evaluate (st with clock := ck + start) mlenv [inner]
-      = evaluate (st' with clock := start) mlenv' [mle']) ∧
-    cont_rel k kv' ∧
-    e_ce_rel e' var' mlenv' kv' mle' ∧
-    env_rel env' mlenv' ∧
-    LIST_REL store_entry_rel store' st'.refs ∧
-    st.ffi = st'.ffi
-Proof
-  Induct_on ‘xs’
-  >> rpt strip_tac
-  >- (
-    qpat_assum ‘cont_rel _ _’ $ irule_at (Pat ‘cont_rel _ _’)
-    >> Cases_on ‘xp’
-    >> gvs[proc_ml_def] >- (
-      Cases_on ‘vs’
-      >> gvs[parameterize_def] >- (
-        simp[Ntimes evaluate_def 3]
-        >> simp[can_pmatch_all_def, evaluate_match_def, vcons_list_def,
-          pmatch_def]
-        >> qpat_assum ‘scheme_env mlenv’ $ simp o single
-          o SRULE [scheme_env_def]
-        >> simp[same_type_def, same_ctor_def, pat_bindings_def]
-        >> simp[GSYM eval_eq_def]
-        >> irule_at (Pos hd) eval_eq_trivial
-        >> simp[Once e_ce_rel_cases]
-      )
-      >> simp[Ntimes evaluate_def 3]
-      >> simp[can_pmatch_all_def, evaluate_match_def, vcons_list_def,
-        pmatch_def]
-      >> qpat_assum ‘scheme_env mlenv’ $ simp o single
-        o SRULE [scheme_env_def]
-      >> simp[same_type_def, same_ctor_def, pat_bindings_def]
-      >> simp[GSYM eval_eq_def]
-      >> irule_at (Pos hd) eval_eq_trivial
-      >> simp[Once e_ce_rel_cases]
-      >> simp[env_rel_cases, FEVERY_FEMPTY]
-    )
-    >> gvs[parameterize_def]
-    >> simp[Ntimes evaluate_def 3]
-    >> simp[can_pmatch_all_def, evaluate_match_def, vcons_list_def,
-      pmatch_def, do_con_check_def, build_conv_def]
-    >> qpat_assum ‘scheme_env mlenv’ $ simp o single
-      o SRULE [scheme_env_def]
-    >> simp[same_type_def, same_ctor_def, pat_bindings_def]
-    >> simp[Ntimes evaluate_def 2, do_app_def, store_alloc_def]
-    >> simp[can_pmatch_all_def, evaluate_match_def, vcons_list_def,
-      pmatch_def, do_con_check_def, build_conv_def, nsOptBind_def]
-    >> qpat_assum ‘scheme_env mlenv’ $ simp o single
-      o SRULE [scheme_env_def]
-    >> simp[GSYM eval_eq_def]
-    >> irule_at (Pos hd) eval_eq_trivial
-    >> simp[]
-    >> rpt (pairarg_tac >> gvs[])
-    >> gvs[fresh_loc_def, store_entry_rel_cases]
-    >> simp[Once ml_v_vals_cases]
-    >> simp[Once e_ce_rel_cases]
-    >> irule_at Any EQ_REFL
-    >> simp[]
-    >> gvs[scheme_env_def, env_rel_cases]
-    >> Cases_on ‘x ∈ FDOM env’ >- (
-      simp[FEVERY_DEF]
-      >> strip_tac
-      >> Cases_on ‘x = x'’
-      >> gvs[] >- (
-        drule $ cj 1 $ iffLR EVERY2_EVERY
-        >> simp[]
-      )
-      >> strip_tac
-      >> gvs[FEVERY_DEF]
-      >> simp[FAPPLY_FUPDATE_THM]
-    )
-    >> irule $ cj 2 FEVERY_STRENGTHEN_THM
-    >> simp[]
-    >> drule_then assume_tac $ cj 1 $ iffLR EVERY2_EVERY
-    >> simp[FEVERY_DEF]
-    >> rpt strip_tac
-    >> ‘x ≠ x'’ by (strip_tac >> gvs[])
-    >> gvs[FEVERY_DEF]
-  )
-  >> gvs[proc_ml_def]
-  >> rpt (pairarg_tac >> gvs[])
-  >> Cases_on ‘vs’
-  >> gvs[parameterize_def] >- (
-    qpat_assum ‘cont_rel _ _’ $ irule_at (Pat ‘cont_rel _ _’)
-    >> simp[Ntimes evaluate_def 3]
-    >> simp[can_pmatch_all_def, evaluate_match_def, vcons_list_def,
-      pmatch_def]
-    >> qpat_assum ‘scheme_env mlenv’ $ simp o single
-      o SRULE [scheme_env_def]
-    >> simp[same_type_def, same_ctor_def, pat_bindings_def]
-    >> simp[GSYM eval_eq_def]
-    >> irule_at (Pos hd) eval_eq_trivial
-    >> simp[Once e_ce_rel_cases]
-    >> simp[env_rel_cases, FEVERY_FEMPTY]
-  )
-  >> simp[Ntimes evaluate_def 3]
-  >> simp[can_pmatch_all_def, evaluate_match_def, vcons_list_def,
-    pmatch_def]
-  >> qpat_assum ‘scheme_env mlenv’ $ simp o single
-    o SRULE [scheme_env_def]
-  >> simp[same_type_def, same_ctor_def, pat_bindings_def]
-  >> simp[Ntimes evaluate_def 4, do_app_def, store_alloc_def]
-  >> simp[can_pmatch_all_def, evaluate_match_def, vcons_list_def,
-    pmatch_def, do_con_check_def, build_conv_def, nsOptBind_def]
-  >> qpat_assum ‘scheme_env mlenv’ $ simp o single
-    o SRULE [scheme_env_def]
-  >> simp[same_type_def, same_ctor_def, pat_bindings_def]
-  >> ‘st.ffi = (st with <|refs :=
-                  st.refs ++ [Refv (Conv (SOME (TypeStamp "Some" 2)) [y])];
-                ffi := st.ffi|>).ffi’ by simp[]
-  >> first_assum $ once_asm_rewrite_tac o single
-  >> pop_assum $ simp_tac pure_ss o single o Once o GSYM
-  >> last_x_assum irule
-  >> simp[]
-  >> rpt (pairarg_tac >> gvs[])
-  >> rpt $ irule_at Any EQ_REFL
-  >> simp[]
-  >> qpat_assum ‘scheme_env mlenv’ $ simp
-    o curry ((::) o swap) [scheme_env_def]
-    o SRULE [scheme_env_def]
-  >> gvs[fresh_loc_def]
-  >> simp[SNOC_APPEND, store_entry_rel_cases]
-  >> irule_at (Pos hd) EVERY_MONOTONIC
-  >> qpat_assum ‘EVERY _ store’ $ irule_at (Pos $ el 2)
-  >> strip_tac >- (
-    rpt strip_tac
-    >> irule OPTION_ALL_MONO
-    >> pop_assum $ irule_at (Pos last)
-    >> rpt strip_tac
-    >> irule valid_val_larger_store
-    >> pop_assum $ irule_at (Pos last)
-    >> simp[]
-  )
-  >> irule_at (Pos hd) valid_val_larger_store
-  >> qpat_assum ‘valid_store _ h'’ $ irule_at (Pos $ el 2)
-  >> simp[]
-  >> irule_at (Pos hd) EVERY_MONOTONIC
-  >> qpat_assum ‘EVERY _ t’ $ irule_at (Pos $ el 2)
-  >> strip_tac >- (
-    rpt strip_tac
-    >> irule valid_val_larger_store
-    >> pop_assum $ irule_at (Pos last)
-    >> simp[]
-  )
-  >> irule_at (Pos $ el 3) valid_cont_larger_store
-  >> qpat_assum ‘valid_cont _ k'’ $ irule_at (Pos $ el 2)
-  >> simp[Once valid_val_cases]
-  >> conj_asm1_tac >- (
-    gvs[can_lookup_cases]
-    >> irule $ cj 2 FEVERY_STRENGTHEN_THM
-    >> irule_at (Pos last) FEVERY_MONO
-    >> qpat_assum ‘FEVERY _ env’ $ irule_at (Pos $ el 2)
-    >> simp[]
-    >> PairCases
-    >> simp[]
-  )
-  >> simp[]
-  >> gvs[env_rel_cases]
-  >> strip_tac >- (
-    Cases_on ‘h ∈ FDOM env’ >- (
-      simp[FEVERY_DEF]
-      >> strip_tac
-      >> Cases_on ‘x = h’
-      >> gvs[] >- (
-        drule $ cj 1 $ iffLR EVERY2_EVERY
-        >> simp[]
-      )
-      >> strip_tac
-      >> gvs[FEVERY_DEF]
-      >> simp[FAPPLY_FUPDATE_THM]
-    )
-    >> irule $ cj 2 FEVERY_STRENGTHEN_THM
-    >> simp[]
-    >> drule_then assume_tac $ cj 1 $ iffLR EVERY2_EVERY
-    >> simp[FEVERY_DEF]
-    >> rpt strip_tac
-    >> ‘x ≠ h’ by (strip_tac >> gvs[])
-    >> gvs[FEVERY_DEF]
-  )
-  >> Cases_on ‘xp’
-  >> simp[]
-  >> irule static_scope_mono
-  >> gvs[Once valid_val_cases]
-  >> qpat_assum ‘static_scope _ _’ $ irule_at (Pos last)
-  >> simp[Ntimes INSERT_SING_UNION 2]
-  >> simp[SUBSET_DEF]
-QED
-
-Theorem preservation_of_letrec:
-  ∀ xs inner (st:'ffi state) mlenv store env store' env' .
-    (store', env') = letrec_preinit store env xs ∧
-    env_rel env mlenv ∧
-    LIST_REL store_entry_rel store st.refs ∧
+Theorem letpreinit_ml_eval:
+  ! xs (st:'ffi state) mlenv e .
     scheme_env mlenv
-    ⇒
-    ∃ ck st' mlenv' var' .
-      (∀ start . evaluate (st with clock:=ck+start) mlenv [letpreinit_ml xs inner]
-        = evaluate (st' with clock:=start) mlenv' [inner]) ∧
-      env_rel env' mlenv' ∧
-      LIST_REL store_entry_rel store' st'.refs ∧
-      (∀ x v . (∀ x' . x ≠ "var" ++ x') ∧ nsLookup mlenv.v (Short x) = SOME v
-      ⇒
-      nsLookup mlenv'.v (Short x) = SOME v) ∧
-      scheme_env mlenv' ∧
-      st.ffi = st'.ffi
+    ==>
+    evaluate st mlenv [letpreinit_ml xs e]
+    =
+    evaluate
+      (st with refs := st.refs ++ (GENLIST (K $ Refv $ Conv (SOME $ scheme_typestamp "None") []) $ LENGTH xs))
+      (letpreinit_mlenv mlenv xs $ LENGTH st.refs)
+      [e]
 Proof
   Induct
-  >> simp[letrec_preinit_def, letpreinit_ml_def]
-  >> rpt strip_tac >- (
-    simp[GSYM eval_eq_def]
-    >> irule_at (Pos hd) eval_eq_trivial
-    >> simp[]
-  )
-  >> rpt (pairarg_tac >> gvs[])
-  >> simp[Ntimes evaluate_def 3, do_con_check_def, build_conv_def,
-    do_app_def, store_alloc_def, nsOptBind_def]
-  >> qpat_assum ‘scheme_env _’ $ simp o single
-    o SRULE [scheme_env_def]
-  >> qsuff_tac ‘∀ mlenv' .
-          (∀x v.
-             (∀x'. x ≠ STRING #"v" (STRING #"a" (STRING #"r" x'))) ∧
-             nsLookup (mlenv with
-               v :=
-                 nsBind (STRING #"v" (STRING #"a" (STRING #"r" (explode h))))
-                   (Loc T (LENGTH st.refs)) mlenv.v).v (Short x) = SOME v ⇒
-             nsLookup mlenv'.v (Short x) = SOME v)
-          ⇔
-          (∀x v.
-             (∀x'. x ≠ STRING #"v" (STRING #"a" (STRING #"r" x'))) ∧
-             nsLookup mlenv.v (Short x) = SOME v ⇒
-             nsLookup mlenv'.v (Short x) = SOME v)
-        ’ >- (
-    strip_tac
-    >> pop_assum $ simp_tac pure_ss o single o GSYM
-    >> ‘st.ffi = (st with <|refs :=
-                    st.refs ++ [Refv (Conv (SOME (TypeStamp "None" 2)) [])];
-                  ffi := st.ffi|>).ffi’ by simp[]
-    >> first_assum $ once_asm_rewrite_tac o single
-    >> pop_assum $ simp_tac pure_ss o single o Once o GSYM
-    >> last_x_assum $ irule
-    >> simp[]
-    >> strip_tac >- gvs[scheme_env_def]
-    >> irule_at (Pos hd) EQ_REFL
-    >> gvs[env_rel_cases, fresh_loc_def, store_entry_rel_cases]
-    >> Cases_on ‘h ∈ FDOM env’ >- (
-      simp[FEVERY_DEF]
-      >> strip_tac
-      >> Cases_on ‘x = h’
-      >> gvs[] >- (
-        drule $ cj 1 $ iffLR EVERY2_EVERY
-        >> simp[]
-      )
-      >> strip_tac
-      >> gvs[FEVERY_DEF]
-      >> simp[FAPPLY_FUPDATE_THM]
-    )
-    >> irule $ cj 2 FEVERY_STRENGTHEN_THM
-    >> simp[]
-    >> drule_then assume_tac $ cj 1 $ iffLR EVERY2_EVERY
-    >> simp[FEVERY_DEF]
-    >> rpt strip_tac
-    >> ‘x ≠ h’ by (strip_tac >> gvs[])
-    >> gvs[FEVERY_DEF]
-  )
-  >> strip_tac
-  >> iff_tac
+  >> simp[letpreinit_mlenv_def, letpreinit_ml_def, GSYM nsEmpty_def]
   >> rpt strip_tac
-  >> qpat_assum ‘∀ _ _ . _ ∧ _ ⇒ _’ irule
+  >> gvs[letpreinit_mlenv_def]
+  >> simp[evaluate_def, do_con_check_def, build_conv_def,
+    do_app_def, store_alloc_def, nsOptBind_def]
+  >> simp_tac bool_ss [SIMP_RULE bool_ss [Once CONS_APPEND] GENLIST_CONS, APPEND_ASSOC]
   >> simp[]
-  >> qpat_assum ‘∀ _ . _ ≠ _’ $ qspec_then ‘explode h’ assume_tac
+  >> Cases_on `mlenv.v`
+  >> simp_tac bool_ss [nsAppend_def, GSYM APPEND_ASSOC]
+  >> simp_tac bool_ss [GSYM nsAppend_def]
+  >> simp[GSYM nsBind_def]
+  >> pop_assum $ simp o single o GSYM
+  >> `! l . GENLIST SUC l = MAP SUC $ GENLIST I l` by simp[MAP_GENLIST]
+  >> pop_assum $ simp o single
+  >> simp[cj 2 ZIP_MAP, MAP_MAP_o, o_DEF]
+  >> qpat_abbrev_tac `st' = st with refs := _`
+  >> qpat_abbrev_tac `mlenv' = mlenv with v := _`
+  >> last_x_assum $ qspec_then `st'` $
+    qspec_then `mlenv'` $ qspec_then `e` $ assume_tac
+  >> `scheme_env mlenv'` by (unabbrev_all_tac >> rpt scheme_env_tac)
+  >> unabbrev_all_tac
   >> simp[]
-  >> Cases_on ‘mlenv’
-  >> gvs[]
+  >> `! n . SUC n = n + 1` by simp[]
+  >> simp[]
 QED
 
-Theorem preservation_of_letinit:
+Theorem letpreinit_ml_eval[allow_rebind] = SRULE [] letpreinit_ml_eval;
+
+Theorem letpreinit_env_rel:
+  ! mlenv xs env l .
+    env_rel env mlenv
+    ==>
+    env_rel (letrec_preinit_env env xs l) (letpreinit_mlenv mlenv xs l)
+Proof
+  simp[letrec_preinit_env_def, letpreinit_mlenv_def, env_rel_cases]
+  >> gen_tac
+  >> `? mlenvv . mlenv.v = mlenvv` by simp[]
+  >> pop_assum $ simp o single
+  >> qid_spec_tac `mlenvv`
+  >> Induct_on `xs`
+  >> simp[GSYM nsEmpty_def, FUPDATE_LIST]
+  >> rpt strip_tac
+  >> simp[GENLIST_CONS]
+  >> simp[GSYM FUPDATE_LIST]
+  >> Cases_on `mlenvv`
+  >> simp_tac bool_ss [nsAppend_def, GSYM APPEND_ASSOC]
+  >> simp[GSYM nsAppend_def, GSYM nsBind_def]
+  >> `! l . GENLIST SUC l = MAP SUC $ GENLIST I l` by simp[MAP_GENLIST]
+  >> pop_assum $ simp o single
+  >> simp[cj 2 ZIP_MAP, MAP_MAP_o, o_DEF]
+  >> `! x y . x + SUC y = SUC x + y` by simp[]
+  >> pop_assum $ simp_tac bool_ss o single
+  >> last_x_assum irule
+  >> gvs[FEVERY_DEF, SPECIFICATION]
+  >> rename1 `_ |+ (x,l)`
+  >> qx_gen_tac `x'`
+  >> Cases_on `x' = x`
+  >> simp[FAPPLY_FUPDATE_THM]
+QED
+
+fun dup n x = if n = 0 then [] else x::dup (n-1) x;
+
+fun reduce_to_cps ck (thms:thm list) = EVERY (dup ck $ qrefine ‘ck+1’)
+    >> simp([GSYM exp_eval_def, GSYM val_eval_def, GSYM ex_eval_def, do_opapp_def, evaluate_def,
+            do_con_check_def, build_conv_def, dec_clock_def, nsOptBind_def,
+            do_app_def, can_pmatch_all_def, pmatch_def, store_lookup_def,
+            same_type_def, same_ctor_def, pat_bindings_def, store_assign_def, store_v_same_type_def]
+         @ thms)
+    >> simp([exp_eval_def, val_eval_def, ex_eval_def] @ thms);
+
+Theorem letinit_preservation:
   ∀ (st:'ffi state) mlenv mlvs store env e k kv var xvs ts .
     EVERY (FDOM env) (MAP FST xvs) ∧
     EVERY (valid_val store) (MAP SND xvs) ∧
@@ -1601,8 +605,7 @@ Theorem preservation_of_letinit:
               (ZIP (MAP FST xvs,MAP (Var ∘ Short) ts))
               (App Opapp [cps_transform e; Var (Short var)])] =
          evaluate (st' with clock := start) mlenv' [mle']) ∧
-      cont_rel k kv' ∧ e_ce_rel (Exp e) var' mlenv' kv' mle' ∧
-      env_rel env mlenv' ∧
+      cont_rel k kv' ∧ cps_rel (Exp env e) var' mlenv' kv' mle' ∧
       LIST_REL store_entry_rel (letinit store env xvs) st'.refs ∧
       st.ffi = st'.ffi
 Proof
@@ -1611,77 +614,54 @@ Proof
   >> gvs[letinit_ml_def, letinit_def] >- (
     simp[GSYM eval_eq_def]
     >> irule_at (Pos hd) eval_eq_trivial
-    >> simp[Once e_ce_rel_cases]
+    >> simp[Once cps_rel_cases]
   )
   >> PairCases_on ‘h’
   >> simp[letinit_def]
   >> gvs[]
-  >> simp[Ntimes evaluate_def 6, do_con_check_def, build_conv_def,
-    nsOptBind_def]
-  >> qpat_assum ‘scheme_env _’ $ simp o single
-    o SRULE [scheme_env_def]
   >> qpat_assum ‘env_rel env _’ $ drule_then assume_tac
     o SRULE [env_rel_cases, FEVERY_DEF, SPECIFICATION]
-  >> simp[do_app_def, store_assign_def, store_v_same_type_def]
-  >> qpat_assum ‘can_lookup env _’ $ drule_then assume_tac
+  >> qpat_assum ‘can_lookup env _’ $ drule
     o SRULE [can_lookup_cases, FEVERY_DEF, SPECIFICATION]
+  >> strip_tac
   >> drule_then assume_tac EVERY2_LENGTH
   >> drule_all_then assume_tac $ cj 2 $ iffLR LIST_REL_EL_EQN
   >> gvs[store_entry_rel_cases]
-  >> (‘st.ffi = (st with <|refs := LUPDATE (Refv (Conv (SOME (TypeStamp "Some" 2)) [y]))
-                      (env ' h0) st.refs; ffi := st.ffi|>).ffi’ by simp[]
-  >> first_assum $ once_asm_rewrite_tac o single
-  >> pop_assum $ simp_tac pure_ss o single o Once o GSYM
-  >> last_x_assum $ irule
-  >> first_assum $ irule_at (Pos last)
+  >> (reduce_to_cps 0 []
+  >> qpat_abbrev_tac `newst = st with refs := _`
+  >> `st.ffi = newst.ffi` by (unabbrev_all_tac >> simp[])
+  >> pop_assum $ simp o single
+  >> last_x_assum irule
+  >> unabbrev_all_tac
+  >> first_assum $ irule_at $ Pos last
   >> simp[]
   >> irule_at (Pos hd) EVERY_MONOTONIC
-  >> last_assum $ irule_at (Pos $ el 2)
+  >> last_assum $ irule_at $ Pat `EVERY _ _`
   >> strip_tac >- (
     rpt strip_tac
-    >> irule valid_val_larger_store
-    >> pop_assum $ irule_at (Pos last)
-    >> simp[LENGTH_LUPDATE]
+    >> irule valid_val_LUPDATE_same
+    >> simp[]
   )
-  >> gvs[can_lookup_cases]
+  >> gvs[can_lookup_LUPDATE_same]
   >> irule EVERY2_LUPDATE_same
   >> simp[store_entry_rel_cases])
 QED
 
-Theorem state_ffi_trivial[simp]:
-  ! st:'ffi state . st with ffi := st.ffi = st
-Proof
-  simp[state_component_equality]
-QED
-
-Theorem state_refs_trivial[simp]:
-  ! st:'ffi state . st with refs := st.refs = st
-Proof
-  simp[state_component_equality]
-QED
-
-fun dup n x = if n = 0 then [] else x::dup (n-1) x;
-
-fun reduce_to_cps ck (thms:thm list) = EVERY (dup ck $ qrefine ‘ck+1’)
-    >> simp([GSYM exp_eval_def, GSYM val_eval_def, GSYM ex_eval_def, do_opapp_def, evaluate_def,
-            do_con_check_def, build_conv_def, dec_clock_def, nsOptBind_def,
-            do_app_def, can_pmatch_all_def, pmatch_def, store_lookup_def,
-            same_type_def, same_ctor_def, pat_bindings_def, store_assign_def, store_v_same_type_def]
-         @ thms)
-    >> simp([exp_eval_def, val_eval_def, ex_eval_def] @ thms);
-
 Theorem application_preservation:
-  ∀ sst sst' env env' fn vs e' ks ks' (st : 'ffi state) t mlfn ts mlvs mlenv k kv mle .
-    application sst ks fn vs = (sst',ks',e') ∧
-    cont_rel st.refs ks kv ∧
-    store_rel sst st.refs ∧
+  ∀ store store' env env' fn vs e' ks ks' (st : 'ffi state) t mlfn ts mlvs mlenv k kv mle .
+    application store ks fn vs = (store',ks',e') ∧
+    valid_val store fn ∧
+    EVERY (valid_val store) vs ∧
+    valid_cont store ks ∧
+    cont_rel ks kv ∧
+    LIST_REL store_entry_rel store st.refs ∧
     nsLookup mlenv.v (Short k) = SOME kv ∧
-    ml_v_vals st.refs fn mlfn ∧
+    ml_v_vals fn mlfn ∧
     nsLookup mlenv.v (Short t) = SOME mlfn ∧
-    LIST_REL (ml_v_vals st.refs) vs mlvs ∧
+    LIST_REL ml_v_vals vs mlvs ∧
     LIST_REL (λx mlv. nsLookup mlenv.v (Short x) = SOME mlv) ts mlvs ∧
     scheme_env mlenv ∧
-    env_rel st.refs env mlenv
+    env_rel env mlenv
     ⇒
     ∃ ck st' mlenv' k' kv' mle' .
       (∀ start . evaluate (st with clock := start + ck) mlenv
@@ -1692,9 +672,9 @@ Theorem application_preservation:
           cons_list (MAP (Var o Short) ts)]]
       =
       evaluate (st' with clock := start) mlenv' [mle']) ∧
-      cont_rel st'.refs ks' kv' ∧
-      cps_rel st'.refs e' k' mlenv' kv' mle'∧
-      store_rel sst' st'.refs ∧
+      cont_rel ks' kv' ∧
+      cps_rel e' k' mlenv' kv' mle'∧
+      LIST_REL store_entry_rel store' st'.refs ∧
       st.ffi = st'.ffi
 Proof
   rpt strip_tac
@@ -1703,9 +683,8 @@ Proof
   >> strip_tac
   >> gvs[Once ml_v_vals_cases]
   >> qrefine ‘ck+3’
-  >> simp[evaluate_def]
-  >> simp[do_opapp_def, dec_clock_def]
-  >> simp[Ntimes find_recfun_def 2, Ntimes build_rec_env_def 2]
+  >> simp[Ntimes evaluate_def 10, do_opapp_def, dec_clock_def,
+       Ntimes find_recfun_def 2, Ntimes build_rec_env_def 2]
   >> simp[Ntimes evaluate_def 3]
   >> simp[can_pmatch_all_def, pmatch_def, nsLookup_def,
     same_type_def, same_ctor_def, evaluate_match_def,
@@ -1770,13 +749,234 @@ Proof
     >> simp[Once cps_rel_cases]
     >> first_assum $ irule_at $ Pos hd
   )
-  >~ [`Prim SMul`] >- cheat
-  >~ [`Prim SMinus`] >- cheat
-  >~ [`Prim SEqv`] >- cheat
-  >~ [`Prim CallCC`] >- cheat
-  >~ [`Prim Cons`] >- cheat
-  >~ [`Prim Car`] >- cheat
-  >~ [`Prim Cdr`] >- cheat
+  >~ [`Prim SMul`] >- (
+    drule $ cj 3 $ iffLR scheme_env_app_def
+    >> strip_tac
+    >> gvs[application_def]
+    >> qrefine ‘ck+2’
+    >> simp[evaluate_def]
+    >> simp[do_opapp_def, dec_clock_def]
+    >> simp[Ntimes find_recfun_def 2, Ntimes build_rec_env_def 2]
+    >> simp[Ntimes evaluate_def 2]
+    >> `? n . 1:int = n` by simp[]
+    >> pop_assum $ simp_tac std_ss o single
+    >> rpt $ pop_assum mp_tac
+    >> qid_spec_tac `n`
+    >> qid_spec_tac `vs`
+    >> qid_spec_tac `ts`
+    >> Induct_on `mlvs`
+    >> rpt strip_tac >- (
+      fs[cons_list_def, vcons_list_def, smul_def]
+      >> rpt strip_tac
+      >> reduce_to_cps 0 [can_pmatch_all_def, pmatch_def, nsLookup_def,
+        same_type_def, same_ctor_def, evaluate_match_def,
+        pat_bindings_def]
+      >> simp[GSYM eval_eq_def]
+      >> irule_at (Pos hd) eval_eq_trivial
+      >> simp[Once cps_rel_cases, Once ml_v_vals_cases]
+    )
+    >> Cases_on `vs`
+    >> fs[]
+    >> Cases_on `ts`
+    >> fs[cons_list_def, vcons_list_def]
+    >> simp[Ntimes evaluate_def 2]
+    >> simp[can_pmatch_all_def, pmatch_def, nsLookup_def,
+      same_type_def, same_ctor_def, evaluate_match_def,
+      pat_bindings_def]
+    >> fs[Once ml_v_vals_cases]
+    >~ [`SNum i`]
+    >> simp[Ntimes evaluate_def 2]
+    >> simp[can_pmatch_all_def, pmatch_def, nsLookup_def,
+      same_type_def, same_ctor_def, evaluate_match_def,
+      pat_bindings_def]
+    >- (
+      qrefine ‘ck+3’
+      >> simp[evaluate_def]
+      >> simp[do_opapp_def, do_app_def, dec_clock_def, opn_lookup_def]
+      >> simp[Ntimes find_recfun_def 2, Ntimes build_rec_env_def 2]
+      >> simp[Ntimes evaluate_def 2]
+      >> simp[smul_def]
+      >> simp[Once INT_MUL_COMM]
+      >> last_x_assum irule
+      >> simp[]
+      >> last_assum $ irule_at $ Pos last
+      >> irule cons_list_val
+      >> simp[]
+    )
+    >> simp[smul_def]
+    >> simp[GSYM eval_eq_def]
+    >> irule_at (Pos hd) eval_eq_trivial
+    >> simp[Once cps_rel_cases]
+    >> first_assum $ irule_at $ Pos hd
+  )
+  >~ [`Prim SMinus`] >- (
+    drule $ cj 9 $ iffLR scheme_env_app_def
+    >> strip_tac
+    >> gvs[application_def]
+    >> qrefine ‘ck+1’
+    >> simp[evaluate_def]
+    >> simp[do_opapp_def, dec_clock_def]
+    >> simp[Once evaluate_def]
+    >> Cases_on `mlvs`
+    >> gvs[vcons_list_def] >>> LASTGOAL (
+      rename1 `vcons_list mlvs`
+      >> rename1 `LIST_REL ml_v_vals vs mlvs`
+      >> gvs[Once ml_v_vals_cases] >~ [`SNum i`] >>> HEADGOAL (
+        Cases_on `mlvs = []`
+        >> gvs[vcons_list_def] >>> LASTGOAL (
+          ‘∃ mlv' mlvs' . mlv'::mlvs'=mlvs’ by (Cases_on ‘mlvs’ >> gvs[])
+          >> ‘∃ v' vs' . v'::vs' = vs’ by gvs[]
+          >> first_assum $ simp_tac bool_ss o single o GSYM
+          >> simp[sminus_def]
+          >> pop_assum $ simp_tac bool_ss o single
+          >> simp[Ntimes evaluate_def 2, can_pmatch_all_def, pmatch_def, nsLookup_def,
+            same_type_def, same_ctor_def, evaluate_match_def,
+            pat_bindings_def, opn_lookup_def]
+          >> simp[Ntimes evaluate_def 2, can_pmatch_all_def, pmatch_def, nsLookup_def,
+            same_type_def, same_ctor_def, evaluate_match_def,
+            pat_bindings_def, opn_lookup_def]
+          >> simp[Ntimes evaluate_def 3]
+          >> pop_assum $ simp_tac bool_ss o single o (fn x => Ntimes x 2) o GSYM
+          >> simp[evaluate_match_def, can_pmatch_all_def, pmatch_def, nsLookup_def,
+            same_type_def, same_ctor_def, evaluate_match_def,
+            pat_bindings_def, opn_lookup_def, vcons_list_def]
+          >> pop_assum kall_tac
+          >> qrefine `ck+3`
+          >> simp[Ntimes evaluate_def 3, can_pmatch_all_def, pmatch_def, nsLookup_def,
+            same_type_def, same_ctor_def, evaluate_match_def,
+            pat_bindings_def]
+          >> simp[Ntimes evaluate_def 7, do_opapp_def]
+          >> simp[Ntimes find_recfun_def 2, Ntimes build_rec_env_def 2]
+          >> simp[Ntimes evaluate_def 2, dec_clock_def]
+          >> ‘∃ n . 0i = n’ by simp[]
+          >> pop_assum $ simp o single
+          >> qpat_abbrev_tac `env_sminus' = env_sminus with v := _`
+          >> ‘nsLookup env_sminus'.v (Short "n") = SOME (Litv (IntLit i))’ by (unabbrev_all_tac >> gvs[])
+          >> ‘nsLookup env_sminus'.v (Short "k") = SOME kv’ by (unabbrev_all_tac >> gvs[])
+          >> ‘env_sminus'.c = env_sminus.c’ by (unabbrev_all_tac >> gvs[])
+          >> qpat_x_assum ‘Abbrev _’ kall_tac
+          >> qpat_x_assum ‘! _ . _’ kall_tac
+          >> gvs[]
+          >> qpat_x_assum `LIST_REL (\ _ _ . nsLookup _ _ = _) _ _` kall_tac
+          >> rpt $ pop_assum mp_tac
+          >> qid_spec_tac ‘n’
+          >> qid_spec_tac ‘mlvs’
+          >> qid_spec_tac ‘vs’
+          >> Induct_on `mlvs`
+          >> Cases_on `vs`
+          >> rpt strip_tac
+          >> gvs[vcons_list_def] >- (
+            simp[sadd_def]
+            >> reduce_to_cps 0 [can_pmatch_all_def, pmatch_def, nsLookup_def,
+              same_type_def, same_ctor_def, evaluate_match_def,
+              pat_bindings_def]
+            >> simp[Once evaluate_def]
+            >> reduce_to_cps 1 [can_pmatch_all_def, pmatch_def, nsLookup_def,
+              same_type_def, same_ctor_def, evaluate_match_def,
+              pat_bindings_def, opn_lookup_def]
+            >> simp[GSYM eval_eq_def]
+            >> irule_at (Pos hd) eval_eq_trivial
+            >> simp[Once cps_rel_cases, Once ml_v_vals_cases]
+          )
+          >> gvs[Once ml_v_vals_cases]
+          >~ [‘sadd (SNum m::_) _’] >- (
+            simp[sadd_def, vcons_list_def]
+            >> simp[evaluate_def, do_opapp_def, do_app_def,
+              opn_lookup_def, can_pmatch_all_def, pmatch_def, nsLookup_def,
+              same_type_def, same_ctor_def, evaluate_match_def,
+              pat_bindings_def, do_con_check_def, build_conv_def, dec_clock_def]
+            >> simp[Ntimes find_recfun_def 2, Ntimes build_rec_env_def 2]
+            >> qrefine ‘ck+3’
+            >> simp[Ntimes evaluate_def 2]
+            >> simp[Once INT_ADD_COMM]
+            >> last_x_assum irule
+          )
+        )
+      )
+    )
+    >> reduce_to_cps 0 [can_pmatch_all_def, pmatch_def, nsLookup_def,
+      same_type_def, same_ctor_def, evaluate_match_def,
+      pat_bindings_def, opn_lookup_def]
+    >> simp[sminus_def, sadd_def]
+    >> simp[GSYM eval_eq_def]
+    >> irule_at (Pos hd) eval_eq_trivial
+    >> simp[Once cps_rel_cases, Once ml_v_vals_cases]
+    >> first_assum $ irule_at $ Pos hd
+  )
+  >~ [`Prim SEqv`] >- (
+    drule $ cj 4 $ iffLR scheme_env_app_def
+    >> strip_tac
+    >> gvs[application_def]
+    >> qrefine ‘ck+1’
+    >> simp[evaluate_def]
+    >> simp[do_opapp_def, dec_clock_def]
+    >> simp[Once evaluate_def]
+    >> Cases_on `mlvs`
+    >> Cases_on `vs`
+    >> gvs[vcons_list_def, seqv_def] >>> LASTGOAL (
+      rename1 `vcons_list mlvs`
+      >> rename1 `LIST_REL ml_v_vals vs mlvs`
+      >> simp[Ntimes evaluate_def 2, can_pmatch_all_def, pmatch_def, nsLookup_def,
+        same_type_def, same_ctor_def, evaluate_match_def,
+        pat_bindings_def, opn_lookup_def]
+      >> Cases_on `mlvs`
+      >> Cases_on `vs`
+      >> gvs[vcons_list_def, seqv_def] >>> LASTGOAL (
+        rename1 `vcons_list mlvs`
+        >> rename1 `LIST_REL ml_v_vals vs mlvs`
+        >> simp[Ntimes evaluate_def 2, can_pmatch_all_def, pmatch_def, nsLookup_def,
+          same_type_def, same_ctor_def, evaluate_match_def,
+          pat_bindings_def, opn_lookup_def]
+        >> Cases_on `mlvs`
+        >> Cases_on `vs`
+        >> gvs[vcons_list_def, seqv_def] >- (
+          reduce_to_cps 0 [can_pmatch_all_def, pmatch_def, nsLookup_def,
+            same_type_def, same_ctor_def, evaluate_match_def,
+            pat_bindings_def, opn_lookup_def]
+          >> gvs[Once ml_v_vals_cases]
+          >~ [`SNum n`] >- (
+            gvs[Once ml_v_vals_cases]
+            >> reduce_to_cps 0 [can_pmatch_all_def, pmatch_def, nsLookup_def,
+              do_eq_def, Boolv_def, bool_type_num_def, ctor_same_type_def, lit_same_type_def]
+            >> simp[GSYM eval_eq_def]
+            >> irule_at (Pos hd) eval_eq_trivial
+            >> simp[Once cps_rel_cases, Once ml_v_vals_cases]
+            >> IF_CASES_TAC
+            >> simp[]
+          )
+          >~ [`SBool T`] >- (
+            gvs[Once ml_v_vals_cases]
+            >> reduce_to_cps 0 [can_pmatch_all_def, pmatch_def, nsLookup_def,
+              do_eq_def, Boolv_def, bool_type_num_def, ctor_same_type_def]
+            >> simp[GSYM eval_eq_def]
+            >> irule_at (Pos hd) eval_eq_trivial
+            >> simp[Once cps_rel_cases, Once ml_v_vals_cases]
+          )
+          >~ [`SBool F`] >- (
+            gvs[Once ml_v_vals_cases]
+            >> reduce_to_cps 0 [can_pmatch_all_def, pmatch_def, nsLookup_def,
+              do_eq_def, Boolv_def, bool_type_num_def, ctor_same_type_def]
+            >> simp[GSYM eval_eq_def]
+            >> irule_at (Pos hd) eval_eq_trivial
+            >> simp[Once cps_rel_cases, Once ml_v_vals_cases]
+          )
+          >> reduce_to_cps 0 [can_pmatch_all_def, pmatch_def, nsLookup_def,
+            do_eq_def, Boolv_def, bool_type_num_def, ctor_same_type_def]
+          >> simp[GSYM eval_eq_def]
+          >> irule_at (Pos hd) eval_eq_trivial
+          >> simp[Once cps_rel_cases, Once ml_v_vals_cases]
+          (*At some point I will need to find a way to evaluate a match
+          expression without expanding all val cases, based on non-equality,
+          because these rewrites take far too long*)
+        )
+      )
+    )
+    >> reduce_to_cps 0 [can_pmatch_all_def, vcons_list_def, pmatch_def, nsLookup_def]
+    >> simp[GSYM eval_eq_def]
+    >> irule_at (Pos hd) eval_eq_trivial
+    >> simp[Once cps_rel_cases]
+    >> first_assum $ irule_at $ Pos hd
+  )
   >~ [`Proc se xs xp e`] >- (
     pop_assum kall_tac
     >> pop_assum kall_tac
@@ -1787,24 +987,27 @@ Proof
     >> simp[Once evaluate_def]
     >> gvs[application_def]
     >> rpt (pairarg_tac >> gvs[])
+    >> last_x_assum kall_tac
+    >> last_x_assum kall_tac
+    >> last_x_assum kall_tac
     >> qpat_x_assum `! _._` kall_tac
     >> qpat_x_assum `scheme_env mlenv` kall_tac
-    >> qpat_x_assum `env_rel _ _ mlenv` kall_tac
+    >> qpat_x_assum `env_rel _ mlenv` kall_tac
     >> qpat_x_assum `scheme_env_app _` kall_tac
     >> rpt $ qpat_x_assum `nsLookup mlenv.v _ = _` kall_tac
     >> qpat_x_assum `LIST_REL _ ts _` kall_tac
     >> qpat_abbrev_tac `proc_env' = proc_env with v:= _`
     >> `scheme_env proc_env'` by (unabbrev_all_tac >> rpt scheme_env_tac)
-    >> `env_rel st.refs se proc_env'` by simp[Abbr `proc_env'`]
+    >> `env_rel se proc_env'` by simp[Abbr `proc_env'`]
     >> `nsLookup proc_env'.v (Short "ts") = SOME (vcons_list mlvs)` by simp[Abbr `proc_env'`]
     >> `nsLookup proc_env'.v (Short "k") = SOME kv` by simp[Abbr `proc_env'`]
     >> qpat_x_assum `Abbrev _` kall_tac
     >> qpat_x_assum `scheme_env proc_env` kall_tac
-    >> qpat_x_assum `env_rel _ _ proc_env` kall_tac
+    >> qpat_x_assum `env_rel _ proc_env` kall_tac
     >> rpt $ pop_assum mp_tac
     >> qid_spec_tac `se`
     >> qid_spec_tac `proc_env'`
-    >> qid_spec_tac `sst`
+    >> qid_spec_tac `store`
     >> qid_spec_tac `st`
     >> qid_spec_tac `vs`
     >> qid_spec_tac `mlvs`
@@ -1812,7 +1015,7 @@ Proof
     >> rpt strip_tac
     >> gvs[]
     >- (
-      qpat_assum ‘cont_rel _ _ _’ $ irule_at (Pat ‘cont_rel _ _ _’)
+      first_assum $ irule_at $ Pat ‘cont_rel _ _’
       >> Cases_on ‘xp’
       >~ [`proc_ml _ (SOME _) _`] >- cheat
       >> gvs[proc_ml_def]
@@ -1828,15 +1031,13 @@ Proof
     >> simp[proc_ml_def]
     >> Cases_on ‘vs’
     >> gvs[parameterize_def] >- (
-      qpat_assum ‘cont_rel _ _ _’ $ irule_at (Pat ‘cont_rel _ _ _’)
+      first_assum $ irule_at (Pat ‘cont_rel _ _’)
       >> reduce_to_cps 0 [can_pmatch_all_def, vcons_list_def, pmatch_def]
       >> simp[GSYM eval_eq_def]
       >> irule_at (Pos hd) eval_eq_trivial
       >> simp[Once cps_rel_cases]
     )
-    >> rpt (pairarg_tac >> gvs[])
     >> reduce_to_cps 0 [can_pmatch_all_def, vcons_list_def, pmatch_def, store_alloc_def]
-val _ = (max_print_depth := 50);
     >> qpat_abbrev_tac `new_st = st with refs := new_refs`
     >> `st.ffi = new_st.ffi` by (unabbrev_all_tac >> simp[])
     >> pop_assum $ simp o single
@@ -1845,113 +1046,215 @@ val _ = (max_print_depth := 50);
     >> simp[]
     >> irule_at Any EQ_REFL
     >> rpt scheme_env_tac
+    >> gvs[fresh_loc_def]
     >> first_assum $ irule_at $ Pat `parameterize _ _ _ _ _ _ = _`
-    >> gvs[fresh_loc_def]
-    >> simp[cont_rel_mono]
-    >> strip_tac >- (
-      irule LIST_REL_mono
-      >> last_assum $ irule_at $ Pos last
-      >> rpt strip_tac
-      >> simp[ml_v_vals_mono]
-    )
-    >> strip_tac >- (
-      irule env_rel_alloc
-      >> gvs[env_rel_cases]
-      >> rename1 `explode x`
-      >> Cases_on ‘x ∈ FDOM env’ >- (
-        simp[FEVERY_DEF]
-        >> strip_tac
-        >> rename1 `x' = x`
-        >> Cases_on ‘x' = x’
-        >> gvs[] >- (
-          drule $ cj 1 $ iffLR EVERY2_EVERY
-          >> simp[GSYM muts_loc_alloc_same]
-          >> simp[muts_loc_FILTER]
-        )
-        >> strip_tac
-        >> gvs[FEVERY_DEF]
-        >> simp[FAPPLY_FUPDATE_THM]
-      )
-      >> irule $ cj 2 FEVERY_STRENGTHEN_THM
-      >> simp[]
-      >> drule_then assume_tac $ cj 1 $ iffLR EVERY2_EVERY
-      >> simp[FEVERY_DEF]
-      >> rpt strip_tac
-      >> ‘x ≠ h’ by (strip_tac >> gvs[])
-      >> gvs[FEVERY_DEF]
-    )
-
-    >> qpat_assum ‘scheme_env mlenv’ $ simp
-      o curry ((::) o swap) [scheme_env_def]
-      o SRULE [scheme_env_def]
-    >> gvs[fresh_loc_def]
-    >> simp[SNOC_APPEND, store_entry_rel_cases]
-    >> irule_at (Pos hd) EVERY_MONOTONIC
-    >> qpat_assum ‘EVERY _ store’ $ irule_at (Pos $ el 2)
-    >> strip_tac >- (
-      rpt strip_tac
-      >> irule OPTION_ALL_MONO
-      >> pop_assum $ irule_at (Pos last)
-      >> rpt strip_tac
-      >> irule valid_val_larger_store
-      >> pop_assum $ irule_at (Pos last)
-      >> simp[]
-    )
-    >> irule_at (Pos hd) valid_val_larger_store
-    >> qpat_assum ‘valid_store _ h'’ $ irule_at (Pos $ el 2)
-    >> simp[]
-    >> irule_at (Pos hd) EVERY_MONOTONIC
-    >> qpat_assum ‘EVERY _ t’ $ irule_at (Pos $ el 2)
-    >> strip_tac >- (
-      rpt strip_tac
-      >> irule valid_val_larger_store
-      >> pop_assum $ irule_at (Pos last)
-      >> simp[]
-    )
-    >> irule_at (Pos $ el 3) valid_cont_larger_store
-    >> qpat_assum ‘valid_cont _ k'’ $ irule_at (Pos $ el 2)
-    >> simp[Once valid_val_cases]
-    >> conj_asm1_tac >- (
-      gvs[can_lookup_cases]
-      >> irule $ cj 2 FEVERY_STRENGTHEN_THM
-      >> irule_at (Pos last) FEVERY_MONO
-      >> qpat_assum ‘FEVERY _ env’ $ irule_at (Pos $ el 2)
-      >> simp[]
-      >> PairCases
-      >> simp[]
-    )
-    >> simp[]
+    >> simp[SNOC_APPEND]
+    >> simp[Once store_entry_rel_cases]
+    >> rename1 `env_rel env proc_env'`
     >> gvs[env_rel_cases]
-    >> strip_tac >- (
-      Cases_on ‘h ∈ FDOM env’ >- (
-        simp[FEVERY_DEF]
-        >> strip_tac
-        >> Cases_on ‘x = h’
-        >> gvs[] >- (
-          drule $ cj 1 $ iffLR EVERY2_EVERY
-          >> simp[]
-        )
-        >> strip_tac
-        >> gvs[FEVERY_DEF]
-        >> simp[FAPPLY_FUPDATE_THM]
+    >> rename1 `explode x`
+    >> Cases_on ‘x ∈ FDOM env’ >- (
+      simp[FEVERY_DEF, SNOC_APPEND]
+      >> strip_tac
+      >> rename1 `x' = x`
+      >> Cases_on ‘x' = x’
+      >> gvs[] >- (
+        irule $ GSYM LIST_REL_LENGTH
+        >> first_assum $ irule_at $ Pos hd
       )
-      >> irule $ cj 2 FEVERY_STRENGTHEN_THM
-      >> simp[]
-      >> drule_then assume_tac $ cj 1 $ iffLR EVERY2_EVERY
-      >> simp[FEVERY_DEF]
-      >> rpt strip_tac
-      >> ‘x ≠ h’ by (strip_tac >> gvs[])
+      >> strip_tac
       >> gvs[FEVERY_DEF]
+      >> simp[FAPPLY_FUPDATE_THM]
     )
-    >> Cases_on ‘xp’
+    >> irule $ cj 2 FEVERY_STRENGTHEN_THM
     >> simp[]
-    >> irule static_scope_mono
-    >> gvs[Once valid_val_cases]
-    >> qpat_assum ‘static_scope _ _’ $ irule_at (Pos last)
-    >> simp[Ntimes INSERT_SING_UNION 2]
-    >> simp[SUBSET_DEF]
+    >> rev_drule_then assume_tac $ LIST_REL_LENGTH
+    >> simp[FEVERY_DEF]
+    >> rpt strip_tac
+    >> ‘x ≠ x'’ by (strip_tac >> gvs[])
+    >> gvs[FEVERY_DEF]
+  )
+  >~ [`Prim CallCC`] >- (
+    gvs[application_def]
+    >> qrefine ‘ck+1’
+    >> simp[evaluate_def]
+    >> simp[do_opapp_def, dec_clock_def]
+    >> simp[Ntimes find_recfun_def 2, Ntimes build_rec_env_def 2]
+    >> simp[Once evaluate_def]
+    >> Cases_on `mlvs`
+    >> Cases_on `vs`
+    >> gvs[vcons_list_def] >>> LASTGOAL (
+      rename1 `vcons_list mlvs`
+      >> rename1 `LIST_REL ml_v_vals vs mlvs`
+      >> simp[Ntimes evaluate_def 2, can_pmatch_all_def, pmatch_def, nsLookup_def,
+        same_type_def, same_ctor_def, evaluate_match_def,
+        pat_bindings_def, opn_lookup_def]
+      >> Cases_on `mlvs`
+      >> Cases_on `vs`
+      >> gvs[vcons_list_def] >- (
+        reduce_to_cps 0 [can_pmatch_all_def, vcons_list_def, pmatch_def, nsLookup_def]
+        >> simp[GSYM eval_eq_def]
+        >> irule_at (Pos hd) eval_eq_trivial
+        >> simp[Once cps_rel_cases, Once ml_v_vals_cases]
+        >> simp[Once cont_rel_cases]
+        >> simp[cps_transform_def, cps_app_ts_def, cons_list_def]
+        >> drule_then assume_tac $ cj 1 $ iffLR scheme_env_app_def
+        >> gvs[scheme_env_def]
+      )
+    )
+    >> reduce_to_cps 0 [can_pmatch_all_def, vcons_list_def, pmatch_def, nsLookup_def]
+    >> simp[GSYM eval_eq_def]
+    >> irule_at (Pos hd) eval_eq_trivial
+    >> simp[Once cps_rel_cases]
+    >> first_assum $ irule_at $ Pos hd
+  )
+  >~ [`Throw ks`] >- (
+    drule $ cj 8 $ iffLR scheme_env_app_def
+    >> strip_tac
+    >> gvs[application_def]
+    >> qrefine ‘ck+1’
+    >> simp[evaluate_def]
+    >> simp[do_opapp_def, dec_clock_def]
+    >> simp[Ntimes find_recfun_def 2, Ntimes build_rec_env_def 2]
+    >> simp[Once evaluate_def]
+    >> Cases_on `mlvs`
+    >> Cases_on `vs`
+    >> gvs[vcons_list_def] >>> LASTGOAL (
+      rename1 `vcons_list mlvs`
+      >> rename1 `LIST_REL ml_v_vals vs mlvs`
+      >> simp[Ntimes evaluate_def 2, can_pmatch_all_def, pmatch_def, nsLookup_def,
+        same_type_def, same_ctor_def, evaluate_match_def,
+        pat_bindings_def, opn_lookup_def]
+      >> Cases_on `mlvs`
+      >> Cases_on `vs`
+      >> gvs[vcons_list_def]
+    )
+    >> reduce_to_cps 0 [can_pmatch_all_def, vcons_list_def, pmatch_def, nsLookup_def]
+    >> simp[GSYM eval_eq_def]
+    >> irule_at (Pos hd) eval_eq_trivial
+    >> simp[Once cps_rel_cases]
+    >> first_assum $ irule_at $ Pos hd
+  )
+  >~ [`Prim Cons`] >- (
+    drule $ cj 5 $ iffLR scheme_env_app_def
+    >> strip_tac
+    >> gvs[application_def]
+    >> qrefine ‘ck+1’
+    >> simp[evaluate_def]
+    >> simp[do_opapp_def, dec_clock_def]
+    >> simp[Once evaluate_def]
+    >> Cases_on `mlvs`
+    >> Cases_on `vs`
+    >> gvs[vcons_list_def] >>> LASTGOAL (
+      rename1 `vcons_list mlvs`
+      >> rename1 `LIST_REL ml_v_vals vs mlvs`
+      >> simp[Ntimes evaluate_def 2, can_pmatch_all_def, pmatch_def, nsLookup_def,
+        same_type_def, same_ctor_def, evaluate_match_def,
+        pat_bindings_def, opn_lookup_def]
+      >> Cases_on `mlvs`
+      >> Cases_on `vs`
+      >> gvs[vcons_list_def] >>> LASTGOAL (
+        rename1 `vcons_list mlvs`
+        >> rename1 `LIST_REL ml_v_vals vs mlvs`
+        >> simp[Ntimes evaluate_def 2, can_pmatch_all_def, pmatch_def, nsLookup_def,
+          same_type_def, same_ctor_def, evaluate_match_def,
+          pat_bindings_def, opn_lookup_def]
+        >> Cases_on `mlvs`
+        >> Cases_on `vs`
+        >> gvs[vcons_list_def] >- (
+          reduce_to_cps 0 [can_pmatch_all_def, vcons_list_def, pmatch_def, store_alloc_def, nsLookup_def]
+          >> gvs[fresh_loc_def]
+          >> simp[GSYM eval_eq_def]
+          >> irule_at (Pos hd) eval_eq_trivial
+          >> simp[Once cps_rel_cases]
+          >> simp[Once ml_v_vals_cases]
+          >> simp[Once store_entry_rel_cases]
+          >> irule $ GSYM LIST_REL_LENGTH
+          >> first_assum $ irule_at $ Pos hd
+        )
+      )
+    )
+    >> reduce_to_cps 0 [can_pmatch_all_def, vcons_list_def, pmatch_def, nsLookup_def]
+    >> gvs[application_def]
+    >> simp[GSYM eval_eq_def]
+    >> irule_at (Pos hd) eval_eq_trivial
+    >> simp[Once cps_rel_cases]
+    >> first_assum $ irule_at $ Pos hd
+  )
+  >~ [`Prim Car`] >- (
+    drule $ cj 6 $ iffLR scheme_env_app_def
+    >> strip_tac
+    >> gvs[application_def]
+    >> qrefine ‘ck+1’
+    >> simp[evaluate_def]
+    >> simp[do_opapp_def, dec_clock_def]
+    >> simp[Once evaluate_def]
+    >> Cases_on `mlvs`
+    >> Cases_on `vs`
+    >> gvs[vcons_list_def] >>> LASTGOAL (
+      rename1 `vcons_list mlvs`
+      >> rename1 `LIST_REL ml_v_vals vs mlvs`
+      >> simp[Ntimes evaluate_def 2, can_pmatch_all_def, pmatch_def, nsLookup_def,
+        same_type_def, same_ctor_def, evaluate_match_def,
+        pat_bindings_def, opn_lookup_def]
+      >> Cases_on `mlvs`
+      >> Cases_on `vs`
+      >> gvs[vcons_list_def] >>> HEADGOAL (
+        rename1 `ml_v_vals v mlv`
+        >> Cases_on `? l . v = PairP l`
+        >> gvs[Once ml_v_vals_cases]
+        >> rfs[Once valid_val_cases] >>> HEADGOAL (
+          drule $ iffLR LIST_REL_EL_EQN
+          >> strip_tac
+          >> pop_assum $ drule_then assume_tac
+          >> gvs[Once store_entry_rel_cases]
+        )
+      )
+    )
+    >> reduce_to_cps 0 [can_pmatch_all_def, vcons_list_def, pmatch_def, nsLookup_def]
+    >> simp[GSYM eval_eq_def]
+    >> irule_at (Pos hd) eval_eq_trivial
+    >> simp[Once cps_rel_cases]
+    >> first_assum $ irule_at $ Pos hd
+  )
+  >~ [`Prim Cdr`] >- (
+    drule $ cj 7 $ iffLR scheme_env_app_def
+    >> strip_tac
+    >> gvs[application_def]
+    >> qrefine ‘ck+1’
+    >> simp[evaluate_def]
+    >> simp[do_opapp_def, dec_clock_def]
+    >> simp[Once evaluate_def]
+    >> Cases_on `mlvs`
+    >> Cases_on `vs`
+    >> gvs[vcons_list_def] >>> LASTGOAL (
+      rename1 `vcons_list mlvs`
+      >> rename1 `LIST_REL ml_v_vals vs mlvs`
+      >> simp[Ntimes evaluate_def 2, can_pmatch_all_def, pmatch_def, nsLookup_def,
+        same_type_def, same_ctor_def, evaluate_match_def,
+        pat_bindings_def, opn_lookup_def]
+      >> Cases_on `mlvs`
+      >> Cases_on `vs`
+      >> gvs[vcons_list_def] >>> HEADGOAL (
+        rename1 `ml_v_vals v mlv`
+        >> Cases_on `? l . v = PairP l`
+        >> gvs[Once ml_v_vals_cases]
+        >> rfs[Once valid_val_cases] >>> HEADGOAL (
+          drule $ iffLR LIST_REL_EL_EQN
+          >> strip_tac
+          >> pop_assum $ drule_then assume_tac
+          >> gvs[Once store_entry_rel_cases]
+        )
+      )
+    )
+    >> reduce_to_cps 0 [can_pmatch_all_def, vcons_list_def, pmatch_def, nsLookup_def]
+    >> simp[GSYM eval_eq_def]
+    >> irule_at (Pos hd) eval_eq_trivial
+    >> simp[Once cps_rel_cases]
+    >> first_assum $ irule_at $ Pos hd
   )
   >> reduce_to_cps 0 []
+  >> gvs[application_def]
   >> simp[GSYM eval_eq_def]
   >> irule_at (Pos hd) eval_eq_trivial
   >> simp[Once cps_rel_cases]
@@ -1959,21 +1262,21 @@ val _ = (max_print_depth := 50);
 QED
 
 Theorem step_preservation:
-  ∀ sst sst' env env' e e' ks ks' (st : 'ffi state) mlenv k kv mle .
-    step (sst, ks, e) = (sst', ks', e') ∧
-    valid_state sst ks e ∧
-    cont_rel st.refs ks kv ∧
-    cps_rel st.refs e k mlenv kv mle ∧
-    store_rel sst st.refs
+  ∀ store store' e e' ks ks' (st : 'ffi state) mlenv k kv mle .
+    step (store, ks, e) = (store', ks', e') ∧
+    valid_state store ks e ∧
+    cont_rel ks kv ∧
+    cps_rel e k mlenv kv mle ∧
+    LIST_REL store_entry_rel store st.refs
     ⇒
     ∃ ck st' mlenv' k' kv' mle' .
       (∀ start . evaluate (st with clock := start + ck) mlenv [mle]
       =
       evaluate (st' with clock := start) mlenv' [mle']) ∧
-      cont_rel st.refs ks' kv' ∧
-      cps_rel st.refs e' k' mlenv' kv' mle' ∧
-      store_rel sst' st'.refs ∧
-      (¬ terminating_state (sst', ks', e') ⇒ 0 < ck) ∧
+      cont_rel ks' kv' ∧
+      cps_rel e' k' mlenv' kv' mle' ∧
+      LIST_REL store_entry_rel store' st'.refs ∧
+      (¬ terminating_state (store', ks', e') ⇒ 0 < ck) ∧
       st.ffi = st'.ffi
 Proof
   Cases_on ‘e’
@@ -1990,87 +1293,95 @@ Proof
     Cases_on ‘e’
     >> simp[step_def, Once cps_rel_cases]
     >~ [‘Letrec bs e’] >- (
-      cheat
-      (*
       Cases_on ‘bs’
       >> rpt strip_tac
-      >> gvs[cps_transform_def] >- (
-        qrefine ‘ck+1’
-        >> simp[SimpLHS, Ntimes evaluate_def 4, do_opapp_def,
-          nsOptBind_def, dec_clock_def, letpreinit_ml_def, letinit_ml_def]
+      >> gvs[cps_transform_def, Excl "MAP"] >- (
+        reduce_to_cps 1 [letpreinit_ml_def, letinit_ml_def]
         >> simp[GSYM eval_eq_def]
         >> irule_at (Pos hd) eval_eq_trivial
-        >> qpat_assum ‘cont_rel _ _’ $ irule_at (Pos hd)
-        >> simp[Once e_ce_rel_cases]
-        >> gvs[scheme_env_def, env_rel_cases]
+        >> first_assum $ irule_at $ Pos hd
+        >> simp[Once cps_rel_cases]
+        >> rpt scheme_env_tac
       )
       >> PairCases_on ‘h’
+      >> gvs[]
       >> simp[cps_transform_def]
       >> rpt (pairarg_tac >> gvs[])
-      >> qrefine ‘ck+1’
-      >> simp[SimpLHS, Ntimes evaluate_def 4, do_opapp_def,
-        nsOptBind_def, dec_clock_def]
-      >> qpat_x_assum ‘letrec_preinit _ _ _ = _’ $ assume_tac o GSYM
-      >> drule preservation_of_letrec
-      >> ‘env_rel env (mlenv with v := nsBind "k" kv mlenv.v)’
-        by gvs[env_rel_cases]
-      >> strip_tac
-      >> pop_assum $ drule_then drule
-      >> ‘scheme_env (mlenv with v := nsBind "k" kv mlenv.v)’
-        by gvs[scheme_env_def]
-      >> strip_tac
-      >> pop_assum $ drule
-      >> strip_tac
-      >> pop_assum $ qspec_then
-        ‘Let (SOME "k'")
-           (Fun "t0"
-              (cps_transform_letinit [(h0,Var (Short "t0"))] t e
-                 (Var (Short "k"))))
-           (App Opapp [cps_transform h1; Var (Short "k'")])’ mp_tac
-      >> rpt strip_tac
-      >> gvs[GSYM eval_eq_def]
-      >> irule_at (Pos hd) eval_eq_trans
-      >> first_assum $ irule_at (Pos hd)
-      >> simp[eval_eq_def]
-      >> simp[Ntimes evaluate_def 2, nsOptBind_def]
+      >> reduce_to_cps 1 [store_alloc_def]
+      >> qpat_abbrev_tac `mlenv' = mlenv with v := _`
+      >> `scheme_env mlenv'` by (unabbrev_all_tac >> rpt scheme_env_tac)
+      >> simp[letpreinit_ml_eval]
+      >> gvs[letrec_preinit_APPEND]
+      >> unabbrev_all_tac
+      >> reduce_to_cps 0 []
       >> simp[GSYM eval_eq_def]
       >> irule_at (Pos hd) eval_eq_trivial
+      >> simp[Once cps_rel_cases]
       >> simp[Once cont_rel_cases]
-      >> qpat_assum ‘cont_rel _ _’ $ irule_at (Pat ‘cont_rel _ _’)
-      >> simp[cps_app_ts_def]
-      >> simp[Once e_ce_rel_cases]
-      >> gvs[scheme_env_def, env_rel_cases]
-      *)
+      >> first_assum $ irule_at $ Pos hd
+      >> drule_then assume_tac LIST_REL_LENGTH
+      >> simp[cps_app_ts_def, letpreinit_env_rel]
+      >> simp[letrec_preinit_env_def, letpreinit_mlenv_def]
+      >> rpt scheme_env_tac
+      >> strip_tac >- (
+        simp[nsLookup_nsAppend_some, id_to_mods_def,
+          nsLookup_def, ALOOKUP_NONE, MEM_MAP]
+        >> disj2_tac
+        >> PairCases
+        >> simp[]
+      )
+      >> strip_tac >- (
+        gvs[scheme_env_def]
+        >> simp[nsLookup_nsAppend_some, id_to_mods_def,
+          nsLookup_def, ALOOKUP_NONE, MEM_MAP]
+        >> first_assum $ irule_at $ Pos hd
+        >> simp[]
+        >> rpt strip_tac
+        >> disj2_tac
+        >> PairCases
+        >> simp[]
+      )
+      >> irule LIST_REL_APPEND_suff
+      >> simp[LIST_REL_EL_EQN, Once store_entry_rel_cases]
     )
     >~ [‘Letrecstar bs e’] >- (
-      cheat
-      (*
-      simp[Once cps_transform_def]
+      simp[cps_transform_def]
       >> rpt strip_tac
       >> rpt (pairarg_tac >> gvs[])
-      >> qrefine ‘ck+1’
-      >> simp[Ntimes evaluate_def 4, do_opapp_def, dec_clock_def]
-      >> pop_assum $ assume_tac o GSYM
-      >> drule preservation_of_letrec
-      >> ‘env_rel env (mlenv with v := nsBind "k" kv mlenv.v)’
-        by gvs[env_rel_cases]
-      >> strip_tac
-      >> pop_assum $ drule_then drule
-      >> ‘scheme_env (mlenv with v := nsBind "k" kv mlenv.v)’
-        by gvs[scheme_env_def]
-      >> strip_tac
-      >> pop_assum $ drule
-      >> strip_tac
-      >> pop_assum $ qspec_then
-        ‘App Opapp
-          [cps_transform (Begin (MAP (UNCURRY Set) bs) e);
-           Var (Short "k")]’ mp_tac
-      >> rpt strip_tac
-      >> gvs[GSYM eval_eq_def]
-      >> first_assum $ irule_at (Pos hd)
-      >> qpat_assum ‘cont_rel _ _’ $ irule_at (Pos hd)
-      >> simp[Once e_ce_rel_cases]
-      *)
+      >> reduce_to_cps 1 [store_alloc_def]
+      >> qpat_abbrev_tac `mlenv' = mlenv with v := _`
+      >> `scheme_env mlenv'` by (unabbrev_all_tac >> rpt scheme_env_tac)
+      >> simp[letpreinit_ml_eval]
+      >> gvs[letrec_preinit_APPEND]
+      >> unabbrev_all_tac
+      >> simp[GSYM eval_eq_def]
+      >> irule_at (Pos hd) eval_eq_trivial
+      >> simp[Once cps_rel_cases]
+      >> first_assum $ irule_at $ Pos hd
+      >> simp[cps_transform_def]
+      >> drule_then assume_tac LIST_REL_LENGTH
+      >> simp[letpreinit_env_rel]
+      >> simp[letrec_preinit_env_def, letpreinit_mlenv_def]
+      >> strip_tac >- (
+        simp[nsLookup_nsAppend_some, id_to_mods_def,
+          nsLookup_def, ALOOKUP_NONE, MEM_MAP]
+        >> disj2_tac
+        >> PairCases
+        >> simp[]
+      )
+      >> strip_tac >- (
+        gvs[scheme_env_def]
+        >> simp[nsLookup_nsAppend_some, id_to_mods_def,
+          nsLookup_def, ALOOKUP_NONE, MEM_MAP]
+        >> first_assum $ irule_at $ Pos hd
+        >> simp[]
+        >> rpt strip_tac
+        >> disj2_tac
+        >> PairCases
+        >> simp[]
+      )
+      >> irule LIST_REL_APPEND_suff
+      >> simp[LIST_REL_EL_EQN, Once store_entry_rel_cases]
     )
     >~ [‘Begin es e’] >>> HEADGOAL $ Cases_on ‘es’
     >> simp[cps_transform_def]
@@ -2085,17 +1396,20 @@ Proof
       gvs[Once valid_state_cases]
       >> gvs[Once static_scope_def]
       >> gvs[Once $ GSYM SPECIFICATION]
-      >> qpat_assum ‘env_rel _ _ _’ $ drule_then assume_tac
+      >> qpat_assum ‘env_rel _ _’ $ drule_then assume_tac
         o SRULE [env_rel_cases, FEVERY_DEF]
-      >> qpat_assum ‘can_lookup _ _’ $ drule_then assume_tac
+      >> qpat_assum ‘can_lookup _ _’ $ drule
         o SRULE [can_lookup_cases, FEVERY_DEF]
-      >> drule_all muts_rel_loc >> strip_tac
+      >> strip_tac
+      >> drule $ iffLR LIST_REL_EL_EQN
+      >> strip_tac
+      >> pop_assum $ drule_then assume_tac
       >> gvs[store_entry_rel_cases]
     )
     >> reduce_to_cps 1 []
     >> simp[GSYM eval_eq_def]
     >> irule_at (Pos hd) eval_eq_trivial
-    >> TRY $ qpat_assum ‘cont_rel _ _ _’ $ irule_at (Pos hd)
+    >> TRY $ qpat_assum ‘cont_rel _ _’ $ irule_at (Pos hd)
     >> simp[Once cps_rel_cases]
     >> simp[Once ml_v_vals_cases, Once cont_rel_cases]
     >> rpt scheme_env_tac
@@ -2122,7 +1436,7 @@ Proof
       >> reduce_to_cps 1 []
       >> simp[GSYM eval_eq_def]
       >> irule_at (Pos hd) eval_eq_trivial
-      >> qpat_assum ‘cont_rel _ _ _’ $ irule_at (Pos hd)
+      >> qpat_assum ‘cont_rel _ _’ $ irule_at (Pos hd)
       >> simp[Once cps_rel_cases]
       >> scheme_env_tac
     )
@@ -2146,90 +1460,74 @@ Proof
         Once cont_rel_cases, cps_transform_def, cps_app_ts_def]
       >> rpt strip_tac
       >> gvs[Once valid_state_cases, Once valid_cont_cases]
-      >> qpat_assum ‘env_rel _ _ _’ $ drule_then assume_tac
+      >> qpat_assum ‘env_rel _ _’ $ drule_then assume_tac
         o SRULE [env_rel_cases, FEVERY_DEF, SPECIFICATION]
-      >> qpat_assum ‘can_lookup _ _’ $ drule_then assume_tac
+      >> qpat_assum ‘can_lookup _ _’ $ drule
         o SRULE [can_lookup_cases, FEVERY_DEF, SPECIFICATION]
-      >> drule_all muts_rel_loc >> strip_tac
+      >> strip_tac
+      >> drule $ iffLR LIST_REL_EL_EQN
+      >> strip_tac
+      >> pop_assum $ drule_then assume_tac
       >> gvs[store_entry_rel_cases]
       >> simp[Once evaluate_def]
       >> reduce_to_cps 1 []
       >> simp[GSYM eval_eq_def]
       >> irule_at (Pos hd) eval_eq_trivial
       >> simp[]
-      >> qpat_assum ‘cont_rel _ _ _’ $ irule_at (Pos hd)
+      >> qpat_assum ‘cont_rel _ _’ $ irule_at (Pos hd)
       >> simp[Once cps_rel_cases, Once ml_v_vals_cases]
-      >> (strip_tac >- (
-        irule muts_rel_LUPDATE_same
-        >> irule_at (Pos hd) muts_rel_mono
-        >> qpat_assum `muts_rel _ _ _` $ irule_at Any
-        >> rpt strip_tac
-        >> gvs[store_entry_rel_cases, ml_v_vals_LUPDATE_same]
-      )
-      >> irule pairs_rel_LUPDATE_diff
-      >> irule_at (Pos hd) pairs_rel_mono
-      >> qpat_assum `pairs_rel _ _ _` $ irule_at Any
-      >> rpt strip_tac
-      >> simp[store_entry_rel_cases]
-      >> irule_at Any EQ_REFL
-      >> irule_at Any ml_v_vals_LUPDATE_same
-      >> rpt $ first_assum $ irule_at $ Pos hd
-      >> rpt strip_tac
-      >> gvs[Once pair_rel_cases]
-      >> simp[Once pair_rel_cases, ml_v_vals_LUPDATE_same])
+      >> irule EVERY2_LUPDATE_same
+      >> simp[Once store_entry_rel_cases]
     )
     >> Cases_on ‘∃ xvs x bs e . h1 = LetinitK xvs x bs e’ >- (
       gvs[]
       >> Cases_on ‘bs’
       >> rpt strip_tac
-      >> gvs[Once cont_rel_cases, Once e_ce_rel_cases]
+      >> gvs[Once cont_rel_cases, Once cps_rel_cases]
       >> gvs[cps_transform_def, step_def, return_def]
-      >> qrefine ‘ck+1’
-      >> simp[SimpLHS, Ntimes evaluate_def 4, do_opapp_def,
-        nsOptBind_def, dec_clock_def] >- (
+      >> simp[Once evaluate_def]
+      >> reduce_to_cps 1 [] >- (
         gvs[Once valid_state_cases]
-        >> qpat_x_assum ‘valid_cont _ _’ $ mp_tac
-          o SRULE [Once valid_val_cases]
-        >> strip_tac
+        >> gvs[Once valid_cont_cases]
         >> ‘∃ xvs' . (x,v)::xvs = xvs'’ by simp[]
         >> first_assum $ simp_tac bool_ss o single
         >> ‘x::(MAP FST xvs) = MAP FST xvs'’ by gvs[]
         >> simp_tac bool_ss [Once $ cj 3 $ GSYM ZIP_def]
         >> first_assum $ simp_tac bool_ss o single
-        >> ‘Var (Short t')::MAP (Var o Short) ts = MAP (Var o Short) (t'::ts)’ by gvs[]
+        >> drule cps_app_ts_distinct >> strip_tac
+        >> ‘! x xs . Var (Short x)::MAP (Var o Short) xs = MAP (Var o Short) (x::xs)’ by gvs[]
         >> first_assum $ simp_tac bool_ss o single
-        >> irule preservation_of_letinit
+        >> irule letinit_preservation
         >> drule cps_app_ts_distinct
         >> strip_tac
         >> gvs[]
-        >> last_assum $ irule_at (Pos last)
-        >> irule_at (Pos $ el 5) EQ_REFL
+        >> last_assum $ irule_at $ Pos last
+        >> last_assum $ irule_at $ Pos last
+        >> irule_at (Pos last) EQ_REFL
         >> irule_at Any EQ_REFL
-        >> simp[]
+        >> rpt scheme_env_tac
         >> irule_at (Pos last) EVERY2_MEM_MONO
-        >> qpat_assum ‘LIST_REL _ ts mlvs’ $ irule_at (Pat ‘LIST_REL _ ts mlvs’)
-        >> strip_tac >- (
-          PairCases
-          >> simp[]
-          >> rpt strip_tac
-          >> qpat_assum ‘LIST_REL _ ts mlvs’ $ assume_tac
-          >> dxrule_then assume_tac EVERY2_LENGTH
-          >> drule_at_then (Pos $ el 2) assume_tac $ cj 1 MEM_ZIP_MEM_MAP
-          >> gvs[]
-          >> Cases_on ‘x'0 = t'’
-          >> gvs[]
-        )
-        >> gvs[scheme_env_def, env_rel_cases]
+        >> first_assum $ irule_at $ Pat ‘LIST_REL _ _ _’
+        >> PairCases
+        >> simp[]
+        >> rpt strip_tac
+        >> qpat_assum ‘LIST_REL _ ts mlvs’ $ assume_tac
+        >> dxrule_then assume_tac EVERY2_LENGTH
+        >> drule_at_then (Pos $ el 2) assume_tac $ cj 1 MEM_ZIP_MEM_MAP
+        >> gvs[]
+        >> qmatch_goalsub_abbrev_tac `nsLookup (nsBind x1 _ _) (Short x2) = SOME _`
+        >> Cases_on ‘x1 = x2’
+        >> gvs[]
       )
       >> PairCases_on ‘h’
       >> gvs[]
       >> simp[cps_transform_def]
-      >> simp[Ntimes evaluate_def 2, nsOptBind_def]
+      >> reduce_to_cps 0 []
       >> simp[GSYM eval_eq_def]
       >> irule_at (Pos hd) eval_eq_trivial
-      >> simp[Once e_ce_rel_cases, Once cont_rel_cases]
+      >> simp[Once cps_rel_cases, Once cont_rel_cases]
       >> simp_tac bool_ss [Once $ GSYM ZIP_def]
-      >> ‘Var (Short t'')::MAP (Var o Short) ts = MAP (Var o Short) (t''::ts)’ by gvs[]
+      >> ‘! x xs . Var (Short x)::MAP (Var o Short) xs = MAP (Var o Short) (x::xs)’ by gvs[]
       >> first_assum $ simp_tac bool_ss o single
       >> irule_at (Pos hd) EQ_REFL
       >> simp[cps_app_ts_def]
@@ -2239,23 +1537,24 @@ Proof
       >> qpat_assum ‘LIST_REL ml_v_vals _ mlvs’ $ assume_tac
       >> dxrule_then assume_tac EVERY2_LENGTH
       >> gvs[]
-      >> qpat_assum ‘cont_rel _ _’ $ irule_at (Pos hd)
-      >> qpat_assum ‘LIST_REL ml_v_vals _ _’ $ irule_at (Pos $ el 2)
+      >> first_assum $ irule_at $ Pos hd
+      >> first_assum $ irule_at (Pos $ el 2)
       >> drule $ GSYM cps_app_ts_distinct
       >> strip_tac
       >> simp[]
       >> irule_at (Pos hd) EVERY2_MEM_MONO
-      >> qpat_assum ‘LIST_REL _ ts mlvs’ $ irule_at (Pat ‘LIST_REL _ ts mlvs’)
+      >> first_assum $ irule_at (Pat ‘LIST_REL _ ts mlvs’)
       >> strip_tac >- (
         PairCases
         >> simp[]
         >> rpt strip_tac
         >> drule_at_then (Pos $ el 2) assume_tac $ cj 1 MEM_ZIP_MEM_MAP
         >> gvs[]
-        >> Cases_on ‘x'0 = t''’
+        >> qmatch_goalsub_abbrev_tac `nsLookup (nsBind x1 _ _) (Short x2) = SOME _`
+        >> Cases_on ‘x1 = x2’
         >> gvs[]
       )
-      >> gvs[scheme_env_def, env_rel_cases]
+      >> rpt scheme_env_tac
     )
     >> Cases_on ‘∃ e es . h1 = ApplyK NONE (e::es)’ >- (
       gvs[]
@@ -2282,16 +1581,16 @@ Proof
       >> simp[Once cps_rel_cases, Once cont_rel_cases]
       >> simp[PULL_EXISTS]
       >> irule_at (Pos hd) EQ_REFL
-      >> qpat_assum ‘cont_rel _ _ _’ $ irule_at (Pos hd)
+      >> qpat_assum ‘cont_rel _ _’ $ irule_at (Pos hd)
       >> simp[cps_app_ts_def]
       >> rpt (pairarg_tac >> gvs[])
-      >> qpat_assum ‘ml_v_vals _ _ _’ $ irule_at Any
-      >> qpat_assum ‘LIST_REL (ml_v_vals _) _ _’ $ irule_at Any
+      >> qpat_assum ‘ml_v_vals _ _’ $ irule_at Any
+      >> qpat_assum ‘LIST_REL ml_v_vals _ _’ $ irule_at Any
       >> drule $ GSYM cps_app_ts_distinct
       >> strip_tac
       >> simp[]
       >> irule_at (Pos hd) EVERY2_MEM_MONO
-      >> qpat_assum ‘LIST_REL _ ts _’ $ irule_at Any
+      >> first_assum $ irule_at $ Pat ‘LIST_REL _ _ _’
       >> qpat_x_assum ‘LIST_REL _ ts _’ $ assume_tac
       >> drule_then assume_tac EVERY2_LENGTH
       >> strip_tac >- (
@@ -2307,128 +1606,21 @@ Proof
     )
     >> Cases_on ‘h1 = ApplyK NONE []’ >- (
       gvs[]
-      >> simp[step_def, return_def, Once cps_rel_cases, Once cont_rel_cases]
-      >> simp[Once ml_v_vals_cases]
+      >> simp[step_def, return_def]
       >> rpt strip_tac
-      >> gvs[]
+      >> gvs[Once cps_rel_cases, Once cont_rel_cases]
       >> simp[Once evaluate_def]
       >> reduce_to_cps 1 []
-      >> cheat
-
-      >> gvs[application_def, sadd_def, smul_def, sminus_def,
-        seqv_def, cps_transform_def, cons_list_def]
-      >> qrefine ‘ck+2’
-      >> simp[SimpLHS, evaluate_def, do_con_check_def,
-        build_conv_def, do_opapp_def, dec_clock_def]
-      >> qpat_assum ‘scheme_env env''’ $ simp o single
-        o SRULE [scheme_env_def]
-      >> simp[Ntimes find_recfun_def 2, Ntimes build_rec_env_def 2]
-      >> qrefine ‘ck+1’
-      >> simp[Ntimes evaluate_def 3, dec_clock_def]
-      >> simp[can_pmatch_all_def, pmatch_def, nsLookup_def,
-        same_type_def, same_ctor_def, evaluate_match_def,
-        pat_bindings_def]
-      >~ [‘Litv (IntLit i)’] >- (
-        qrefine ‘ck+1’
-        >> simp[Once evaluate_def]
-        >> simp[GSYM eval_eq_def]
-        >> irule_at (Pos hd) eval_eq_trivial
-        >> simp[Once cps_rel_cases]
-        >> last_assum $ irule_at (Pos hd)
-        >> simp[env_rel_cases, FEVERY_FEMPTY]
-      )
-      >~ [‘SOME (Conv (SOME (TypeStamp "SBool" _)) [
-        Conv (Some (TypeStamp "True" _)) []
-      ])’] >- (
-        qrefine ‘ck+1’
-        >> simp[Once evaluate_def]
-        >> simp[GSYM eval_eq_def]
-        >> irule_at (Pos hd) eval_eq_trivial
-        >> simp[Once cps_rel_cases]
-        >> last_assum $ irule_at (Pos hd)
-        >> simp[env_rel_cases, FEVERY_FEMPTY]
-      )
-      >~ [‘SOME (Conv (SOME (TypeStamp "SBool" _)) [
-        Conv (Some (TypeStamp "False" _)) []
-      ])’] >- (
-        qrefine ‘ck+1’
-        >> simp[Once evaluate_def]
-        >> simp[GSYM eval_eq_def]
-        >> irule_at (Pos hd) eval_eq_trivial
-        >> simp[Once cps_rel_cases]
-        >> last_assum $ irule_at (Pos hd)
-        >> simp[env_rel_cases, FEVERY_FEMPTY]
-      )
-      >~ [‘SOME (Conv (SOME (TypeStamp "SList" _)) [_])’] >- (
-        qrefine ‘ck+1’
-        >> simp[Once evaluate_def]
-        >> simp[GSYM eval_eq_def]
-        >> irule_at (Pos hd) eval_eq_trivial
-        >> simp[Once cps_rel_cases]
-        >> last_assum $ irule_at (Pos hd)
-        >> simp[env_rel_cases, FEVERY_FEMPTY]
-      )
-      >~ [‘SOME (Conv (SOME (TypeStamp "Wrong" _)) [_])’] >- (
-        qrefine ‘ck+1’
-        >> simp[Once evaluate_def]
-        >> simp[GSYM eval_eq_def]
-        >> irule_at (Pos hd) eval_eq_trivial
-        >> simp[Once cps_rel_cases]
-        >> last_assum $ irule_at (Pos hd)
-        >> simp[env_rel_cases, FEVERY_FEMPTY]
-      )
-      >> qrefine ‘ck+2’
-      >> simp[evaluate_def]
-      >> simp[do_opapp_def,
-      Once find_recfun_def, Once build_rec_env_def]
-      >> simp[Ntimes evaluate_def 4, dec_clock_def]
-      >> simp[can_pmatch_all_def, pmatch_def, nsLookup_def,
-        same_type_def, same_ctor_def, evaluate_match_def,
-        pat_bindings_def]
-      >~ [‘"SAdd"’] >- (
-        qrefine ‘ck+1’
-        >> simp[Ntimes evaluate_def 3, nsOptBind_def,
-          do_con_check_def, build_conv_def]
-        >> simp[GSYM eval_eq_def]
-        >> irule_at (Pos hd) eval_eq_trivial
-        >> last_assum $ irule_at (Pos hd)
-        >> simp[Once cps_rel_cases, Once ml_v_vals_cases]
-        >> simp[env_rel_cases, FEVERY_FEMPTY]
-      )
-      >~ [‘"SMul"’] >- (
-        qrefine ‘ck+1’
-        >> simp[Ntimes evaluate_def 3, nsOptBind_def,
-          do_con_check_def, build_conv_def]
-        >> simp[GSYM eval_eq_def]
-        >> irule_at (Pos hd) eval_eq_trivial
-        >> last_assum $ irule_at (Pos hd)
-        >> simp[Once cps_rel_cases, Once ml_v_vals_cases]
-        >> simp[env_rel_cases, FEVERY_FEMPTY]
-      )
-      >~ [‘Proc _ _ _ _’] >- (
-        rpt (pairarg_tac >> gvs[])
-        >> irule preservation_of_proc
-        >> simp[]
-        >> qpat_assum ‘scheme_env env'³'’ $ simp
-          o curry ((::) o swap) [scheme_env_def]
-          o SRULE [scheme_env_def]
-        >> first_assum $ irule_at Any o GSYM
-        >> simp[vcons_list_def]
-        >> last_x_assum $ mp_tac o SRULE [Once valid_state_cases]
-        >> strip_tac
-        >> simp[]
-        >> qpat_x_assum ‘valid_cont _ _’ $ mp_tac o SRULE [Once valid_val_cases]
-        >> strip_tac
-        >> simp[]
-        >> qpat_x_assum ‘valid_val _ (Proc _ _ _ _)’ $ mp_tac o SRULE [Once valid_val_cases]
-        >> strip_tac
-        >> gvs[env_rel_cases]
-      )
-      >> simp[GSYM eval_eq_def]
-      >> irule_at (Pos hd) eval_eq_trivial
-      >> simp[Once cps_rel_cases]
-      >> simp[env_rel_cases, FEVERY_FEMPTY]
-      >> last_assum $ irule_at Any
+      >> simp[cps_transform_def]
+      >> simp_tac bool_ss [Once ADD_COMM]
+      >> `cons_list [] = cons_list $ MAP (Var o Short) []` by simp[]
+      >> pop_assum $ simp_tac bool_ss o single
+      >> irule application_preservation
+      >> simp[]
+      >> rpt scheme_env_tac
+      >> rpt $ first_assum $ irule_at $ Pos hd
+      >> gvs[Once valid_state_cases]
+      >> gvs[Once valid_cont_cases]
     )
     >> Cases_on ‘∃ fn vs . h1 = ApplyK (SOME (fn, vs)) []’ >- (
       gvs[]
@@ -2438,353 +1630,29 @@ Proof
       >> simp[Once evaluate_def]
       >> reduce_to_cps 1 [Excl "MAP"]
       >> gvs[cps_transform_def, Excl "MAP"]
-      >> simp_tac std_ss [Once $ GSYM MAP_REVERSE]
-
-      gvs[]
-      >> simp[step_def, return_def, Once e_ce_rel_cases,
-        Once cont_rel_cases]
-      >> rpt strip_tac
-      >> gvs[cps_transform_def, cons_list_def]
-      >> qrefine ‘ck+1’
-      >> simp[evaluate_def, do_con_check_def,
-        build_conv_def, do_opapp_def, dec_clock_def]
-      >> drule $ cps_app_ts_distinct
-      >> strip_tac
-      >> ‘scheme_env (env'' with v:= nsBind t' mlv env''.v)’ by gvs[scheme_env_def]
-      >> qsuff_tac ‘LIST_REL (λx v'. nsLookup (env'' with v:= nsBind t' mlv
-      env''.v).v (Short x) = SOME v') (REVERSE (t'::ts)) (REVERSE (mlv::mlvs))’ >- (
-        strip_tac
-        >> drule_all_then assume_tac cons_list_val
-        >> gvs[Once ml_v_vals_cases]
-        >> gvs[application_def]
-        >> qpat_assum ‘scheme_env env''’ $ simp o single o SRULE [scheme_env_def]
-        >> simp[Ntimes find_recfun_def 2, Ntimes build_rec_env_def 2]
-        >~ [‘Prim SAdd’] >- (
-          qrefine ‘ck+3’
-          >> simp[Ntimes evaluate_def 3]
-          >> simp[can_pmatch_all_def, pmatch_def, nsLookup_def,
-            same_type_def, same_ctor_def, evaluate_match_def,
-            pat_bindings_def]
-          >> simp[Ntimes find_recfun_def 2, Ntimes build_rec_env_def 2]
-          >> simp[Ntimes evaluate_def 3]
-          >> simp[can_pmatch_all_def, pmatch_def, nsLookup_def,
-            same_type_def, same_ctor_def, evaluate_match_def,
-            pat_bindings_def]
-          >> simp[Ntimes evaluate_def 7, do_opapp_def]
-          >> simp[Ntimes find_recfun_def 2, Ntimes build_rec_env_def 2]
-          >> qrefine ‘ck+2’
-          >> simp[Ntimes evaluate_def 2, dec_clock_def]
-          >> irule preservation_of_sadd_body
-          >> simp[]
-          >> irule_at (Pos hd) EQ_REFL
-          >> irule $ cj 1 $ iffLR LIST_REL_APPEND
-          >> simp[]
-        )
-        >~ [‘Prim SMul’] >- (
-          qrefine ‘ck+3’
-          >> simp[Ntimes evaluate_def 3]
-          >> simp[can_pmatch_all_def, pmatch_def, nsLookup_def,
-            same_type_def, same_ctor_def, evaluate_match_def,
-            pat_bindings_def]
-          >> simp[Ntimes find_recfun_def 2, Ntimes build_rec_env_def 2]
-          >> simp[Ntimes evaluate_def 3]
-          >> simp[can_pmatch_all_def, pmatch_def, nsLookup_def,
-            same_type_def, same_ctor_def, evaluate_match_def,
-            pat_bindings_def]
-          >> simp[Ntimes evaluate_def 7, do_opapp_def]
-          >> simp[Ntimes find_recfun_def 2, Ntimes build_rec_env_def 2]
-          >> qrefine ‘ck+2’
-          >> simp[Ntimes evaluate_def 2, dec_clock_def]
-          >> irule preservation_of_smul_body
-          >> simp[]
-          >> simp[scheme_env2_def]
-          >> irule_at (Pos hd) EQ_REFL
-          >> irule $ cj 1 $ iffLR LIST_REL_APPEND
-          >> simp[]
-        )
-        >~ [‘Prim SMinus’] >- (
-          qrefine ‘ck+4’
-          >> simp[Ntimes evaluate_def 3]
-          >> simp[can_pmatch_all_def, pmatch_def, nsLookup_def,
-            same_type_def, same_ctor_def, evaluate_match_def,
-            pat_bindings_def]
-          >> simp[Ntimes evaluate_def 5, do_opapp_def, dec_clock_def]
-          >> simp[can_pmatch_all_def, pmatch_def, nsLookup_def,
-            same_type_def, same_ctor_def, evaluate_match_def,
-            pat_bindings_def]
-          >> irule preservation_of_sminus_body
-          >> simp[]
-          >> simp[scheme_env3_def, scheme_env2_def]
-          >> irule_at (Pos hd) EQ_REFL
-          >> irule $ cj 1 $ iffLR LIST_REL_APPEND
-          >> simp[]
-        )
-        >~ [‘Proc _ _ _ _’] >- (
-          qrefine ‘ck+3’
-          >> simp[Ntimes evaluate_def 3]
-          >> simp[can_pmatch_all_def, pmatch_def, nsLookup_def,
-            same_type_def, same_ctor_def, evaluate_match_def,
-            pat_bindings_def]
-          >> qrefine ‘ck+1’
-          >> simp[Ntimes evaluate_def 5, do_opapp_def, dec_clock_def]
-          >> rpt (pairarg_tac >> gvs[])
-          >> irule preservation_of_proc
-          >> simp[]
-          >> qpat_assum ‘scheme_env env'³'’ $ simp
-            o curry ((::) o swap) [scheme_env_def]
-            o SRULE [scheme_env_def]
-          >> first_assum $ irule_at Any o GSYM
-          >> rpt $ irule_at Any EQ_REFL
-          >> simp[]
-          >> last_x_assum $ mp_tac o SRULE [Once valid_state_cases]
-          >> strip_tac
-          >> simp[]
-          >> qpat_x_assum ‘valid_cont _ _’ $ mp_tac o SRULE [Once valid_val_cases]
-          >> strip_tac
-          >> simp[]
-          >> qpat_x_assum ‘valid_val _ (Proc _ _ _ _)’ $ mp_tac o SRULE [Once valid_val_cases]
-          >> strip_tac
-          >> gvs[env_rel_cases]
-        )
-        >~ [‘Prim SEqv’] >- (
-          qrefine ‘ck+4’
-          >> simp[Ntimes evaluate_def 3]
-          >> simp[can_pmatch_all_def, pmatch_def, nsLookup_def,
-            same_type_def, same_ctor_def, evaluate_match_def,
-            pat_bindings_def]
-          >> simp[Ntimes evaluate_def 5, do_opapp_def, dec_clock_def]
-          >> simp[can_pmatch_all_def, pmatch_def, nsLookup_def,
-            same_type_def, same_ctor_def, evaluate_match_def,
-            pat_bindings_def]
-          >> Cases_on ‘vs’ using SNOC_CASES
-          >> gvs[vcons_list_def, seqv_def] >- (
-            simp[Ntimes evaluate_def 8]
-            >> simp[can_pmatch_all_def, pmatch_def, nsLookup_def,
-              same_type_def, same_ctor_def, evaluate_match_def,
-              pat_bindings_def]
-            >> simp[GSYM eval_eq_def]
-            >> irule_at (Pos hd) eval_eq_trivial
-            >> qpat_assum ‘cont_rel _ _’ $ irule_at (Pos hd)
-            >> simp[Once e_ce_rel_cases, env_rel_cases, FEVERY_FEMPTY]
-          )
-          >> Cases_on ‘mlvs’ using SNOC_CASES
-          >> gvs[vcons_list_def, LIST_REL_SNOC, REVERSE_SNOC]
-          >> simp[Ntimes evaluate_def 5]
-          >> simp[can_pmatch_all_def, pmatch_def, nsLookup_def,
-            same_type_def, same_ctor_def, evaluate_match_def,
-            pat_bindings_def]
-          >> Cases_on ‘l’ using SNOC_CASES
-          >> gvs[vcons_list_def, seqv_def] >- (
-            simp[Ntimes evaluate_def 8]
-            >> simp[can_pmatch_all_def, pmatch_def, nsLookup_def,
-              same_type_def, same_ctor_def, evaluate_match_def,
-              pat_bindings_def]
-            >> Cases_on ‘∃ n . x = SNum n’ >- (
-              gvs[Once ml_v_vals_cases]
-              >> simp[Ntimes evaluate_def 8]
-              >> simp[can_pmatch_all_def, pmatch_def, nsLookup_def,
-                same_type_def, same_ctor_def, evaluate_match_def,
-                pat_bindings_def, do_con_check_def, build_conv_def]
-              >> Cases_on ‘∃ m . v = SNum m’ >- (
-                gvs[Once ml_v_vals_cases]
-                >> simp[Ntimes evaluate_def 11, nsOptBind_def, do_app_def]
-                >> simp[can_pmatch_all_def, pmatch_def, nsLookup_def,
-                  same_type_def, same_ctor_def, evaluate_match_def,
-                  pat_bindings_def, do_con_check_def, build_conv_def,
-                  do_eq_def, lit_same_type_def]
-                >> simp[GSYM eval_eq_def]
-                >> irule_at (Pos hd) eval_eq_trivial
-                >> simp[env_rel_cases, FEVERY_FEMPTY]
-                >> qpat_assum ‘cont_rel _ _’ $ irule_at (Pos hd)
-                >> Cases_on ‘i=i'’
-                >> simp[Once e_ce_rel_cases, Once ml_v_vals_cases,
-                  Boolv_def, bool_type_num_def]
-              )
-              >> Cases_on ‘v’
-              >> gvs[Once ml_v_vals_cases]
-              >> simp[Ntimes evaluate_def 8, nsOptBind_def]
-              >> simp[can_pmatch_all_def, pmatch_def, nsLookup_def,
-                same_type_def, same_ctor_def, evaluate_match_def,
-                pat_bindings_def, do_con_check_def, build_conv_def]
-              >> simp[GSYM eval_eq_def]
-              >> irule_at (Pos hd) eval_eq_trivial
-              >> simp[env_rel_cases, FEVERY_FEMPTY]
-              >> qpat_assum ‘cont_rel _ _’ $ irule_at (Pos hd)
-              >> simp[Once e_ce_rel_cases, Once ml_v_vals_cases,
-                Boolv_def, bool_type_num_def]
-            )
-            >> Cases_on ‘∃ b . x = SBool b’ >- (
-              gvs[Once ml_v_vals_cases]
-              >> simp[Ntimes evaluate_def 8]
-              >> simp[can_pmatch_all_def, pmatch_def, nsLookup_def,
-                same_type_def, same_ctor_def, evaluate_match_def,
-                pat_bindings_def, do_con_check_def, build_conv_def]
-              >> (Cases_on ‘∃ b' . v = SBool b'’ >- (
-                gvs[Once ml_v_vals_cases]
-                >> simp[Ntimes evaluate_def 11, nsOptBind_def, do_app_def]
-                >> simp[can_pmatch_all_def, pmatch_def, nsLookup_def,
-                  same_type_def, same_ctor_def, evaluate_match_def,
-                  pat_bindings_def, do_con_check_def, build_conv_def,
-                  do_eq_def, lit_same_type_def, ctor_same_type_def]
-                >> simp[GSYM eval_eq_def]
-                >> irule_at (Pos hd) eval_eq_trivial
-                >> simp[env_rel_cases, FEVERY_FEMPTY]
-                >> qpat_assum ‘cont_rel _ _’ $ irule_at (Pos hd)
-                >> simp[Once e_ce_rel_cases, Once ml_v_vals_cases,
-                  Boolv_def, bool_type_num_def]
-              ))
-              >> Cases_on ‘v’ >> gvs[]
-              >> gvs[Once ml_v_vals_cases]
-              >> simp[Ntimes evaluate_def 8, nsOptBind_def]
-              >> simp[can_pmatch_all_def, pmatch_def, nsLookup_def,
-                same_type_def, same_ctor_def, evaluate_match_def,
-                pat_bindings_def, do_con_check_def, build_conv_def]
-              >> simp[GSYM eval_eq_def]
-              >> irule_at (Pos hd) eval_eq_trivial
-              >> simp[env_rel_cases, FEVERY_FEMPTY]
-              >> qpat_assum ‘cont_rel _ _’ $ irule_at (Pos hd)
-              >> simp[Once e_ce_rel_cases, Once ml_v_vals_cases,
-                Boolv_def, bool_type_num_def]
-            )
-            >> Cases_on ‘x’ >> gvs[]
-            >> gvs[Once ml_v_vals_cases]
-            >> simp[Ntimes evaluate_def 9, nsOptBind_def]
-            >> simp[can_pmatch_all_def, pmatch_def, nsLookup_def,
-              same_type_def, same_ctor_def, evaluate_match_def,
-              pat_bindings_def, do_con_check_def, build_conv_def]
-            >> simp[GSYM eval_eq_def]
-            >> irule_at (Pos hd) eval_eq_trivial
-            >> simp[env_rel_cases, FEVERY_FEMPTY]
-            >> qpat_assum ‘cont_rel _ _’ $ irule_at (Pos hd)
-            >> simp[Once e_ce_rel_cases, Once ml_v_vals_cases]
-          )
-          >> Cases_on ‘l'’ using SNOC_CASES
-          >> gvs[vcons_list_def, LIST_REL_SNOC, REVERSE_SNOC]
-          >> Cases_on ‘l''’ using SNOC_CASES
-          >> Cases_on ‘l’ using SNOC_CASES
-          >> gvs[vcons_list_def, seqv_def, LIST_REL_SNOC, REVERSE_SNOC]
-          >> simp[Ntimes evaluate_def 8]
-          >> simp[can_pmatch_all_def, pmatch_def, nsLookup_def,
-            same_type_def, same_ctor_def, evaluate_match_def,
-            pat_bindings_def]
-          >> simp[GSYM eval_eq_def]
-          >> irule_at (Pos hd) eval_eq_trivial
-          >> qpat_assum ‘cont_rel _ _’ $ irule_at (Pos hd)
-          >> simp[Once e_ce_rel_cases, env_rel_cases, FEVERY_FEMPTY]
-        )
-        >~ [‘Prim CallCC’] >- (
-          qrefine ‘ck+4’
-          >> simp[Ntimes evaluate_def 5]
-          >> simp[can_pmatch_all_def, pmatch_def, nsLookup_def,
-            same_type_def, same_ctor_def, evaluate_match_def,
-            pat_bindings_def]
-          >> simp[Ntimes find_recfun_def 2, Ntimes build_rec_env_def 2]
-          >> simp[Ntimes evaluate_def 4, do_opapp_def]
-          >> simp[can_pmatch_all_def, pmatch_def, nsLookup_def,
-            same_type_def, same_ctor_def, evaluate_match_def,
-            pat_bindings_def]
-          >> simp[Ntimes find_recfun_def 2, Ntimes build_rec_env_def 2]
-          >> simp[Ntimes evaluate_def 1, do_opapp_def, dec_clock_def]
-          >> simp[can_pmatch_all_def, pmatch_def, nsLookup_def,
-            same_type_def, same_ctor_def, evaluate_match_def,
-            pat_bindings_def]
-          >> simp[Ntimes find_recfun_def 2, Ntimes build_rec_env_def 2]
-          >> Cases_on ‘vs’ using SNOC_CASES
-          >> gvs[vcons_list_def] >- (
-            simp[Ntimes evaluate_def 8]
-            >> simp[can_pmatch_all_def, pmatch_def, nsLookup_def,
-              same_type_def, same_ctor_def, evaluate_match_def,
-              pat_bindings_def]
-            >> simp[Ntimes evaluate_def 5, do_con_check_def, build_conv_def,
-              nsOptBind_def]
-            >> simp[GSYM eval_eq_def]
-            >> irule_at (Pos hd) eval_eq_trivial
-            >> simp[env_rel_cases, FEVERY_FEMPTY]
-            >> simp[Once cont_rel_cases]
-            >> gvs[cps_transform_def, cps_app_ts_def]
-            >> irule_at (Pos hd) EQ_REFL
-            >> qpat_assum ‘cont_rel _ _’ $ irule_at (Pos hd)
-            >> qpat_assum ‘ml_v_vals _ _’ $ irule_at Any
-            >> simp[Once e_ce_rel_cases]
-            >> simp[Once ml_v_vals_cases]
-            >> simp[cons_list_def]
-            >> simp[scheme_env_def, env_rel_cases, FEVERY_FEMPTY]
-          )
-          >> Cases_on ‘mlvs’ using SNOC_CASES
-          >> gvs[vcons_list_def, LIST_REL_SNOC, REVERSE_SNOC]
-          >> Cases_on ‘l’ using SNOC_CASES
-          >> Cases_on ‘l'’ using SNOC_CASES
-          >> gvs[vcons_list_def, LIST_REL_SNOC, REVERSE_SNOC]
-          >> simp[Ntimes evaluate_def 8]
-          >> simp[can_pmatch_all_def, pmatch_def, nsLookup_def,
-            same_type_def, same_ctor_def, evaluate_match_def,
-            pat_bindings_def]
-          >> simp[GSYM eval_eq_def]
-          >> irule_at (Pos hd) eval_eq_trivial
-          >> qpat_assum ‘cont_rel _ _’ $ irule_at (Pos hd)
-          >> simp[Once e_ce_rel_cases, env_rel_cases, FEVERY_FEMPTY]
-        )
-        >~ [‘Throw _’] >- (
-          qrefine ‘ck+4’
-          >> simp[Ntimes evaluate_def 5]
-          >> simp[can_pmatch_all_def, pmatch_def, nsLookup_def,
-            same_type_def, same_ctor_def, evaluate_match_def,
-            pat_bindings_def]
-          >> simp[Ntimes find_recfun_def 2, Ntimes build_rec_env_def 2]
-          >> simp[Ntimes evaluate_def 5, do_opapp_def, dec_clock_def]
-          >> simp[can_pmatch_all_def, pmatch_def, nsLookup_def,
-            same_type_def, same_ctor_def, evaluate_match_def,
-            pat_bindings_def]
-          >> simp[Ntimes find_recfun_def 2, Ntimes build_rec_env_def 2]
-          >> Cases_on ‘vs’ using SNOC_CASES
-          >> gvs[vcons_list_def] >- (
-            simp[Ntimes evaluate_def 8]
-            >> simp[can_pmatch_all_def, pmatch_def, nsLookup_def,
-              same_type_def, same_ctor_def, evaluate_match_def,
-              pat_bindings_def]
-            >> simp[GSYM eval_eq_def]
-            >> irule_at (Pos hd) eval_eq_trivial
-            >> simp[env_rel_cases, FEVERY_FEMPTY]
-            >> qpat_assum ‘cont_rel _ _’ $ irule_at (Pos hd)
-            >> simp[Once e_ce_rel_cases]
-          )
-          >> Cases_on ‘mlvs’ using SNOC_CASES
-          >> gvs[vcons_list_def, LIST_REL_SNOC, REVERSE_SNOC]
-          >> Cases_on ‘l’ using SNOC_CASES
-          >> Cases_on ‘l'’ using SNOC_CASES
-          >> gvs[vcons_list_def, LIST_REL_SNOC, REVERSE_SNOC]
-          >> simp[Ntimes evaluate_def 8]
-          >> simp[can_pmatch_all_def, pmatch_def, nsLookup_def,
-            same_type_def, same_ctor_def, evaluate_match_def,
-            pat_bindings_def]
-          >> simp[GSYM eval_eq_def]
-          >> irule_at (Pos hd) eval_eq_trivial
-          >> qpat_assum ‘cont_rel _ _’ $ irule_at (Pos hd)
-          >> simp[Once e_ce_rel_cases, env_rel_cases, FEVERY_FEMPTY]
-        )
-        >> qrefine ‘ck+3’
-        >> simp[Ntimes evaluate_def 5]
-        >> simp[can_pmatch_all_def, pmatch_def, nsLookup_def,
-          same_type_def, same_ctor_def, evaluate_match_def,
-          pat_bindings_def]
-        >> simp[Once evaluate_def, do_opapp_def, dec_clock_def,
-          do_con_check_def, build_conv_def]
-        >> simp[GSYM eval_eq_def]
-        >> irule_at (Pos hd) eval_eq_trivial
-        >> simp[env_rel_cases, FEVERY_FEMPTY]
-        >> qpat_assum ‘cont_rel _ _’ $ irule_at (Pos hd)
-        >> simp[Once e_ce_rel_cases]
-      )
+      >> simp_tac bool_ss [GSYM MAP_REVERSE, Excl "MAP"]
+      >> simp_tac bool_ss [Once ADD_COMM]
+      >> irule application_preservation
       >> simp[]
-      >> irule_at (Pos hd) EVERY2_MEM_MONO
-      >> qpat_assum ‘LIST_REL _ ts _’ $ irule_at Any
+      >> drule cps_app_ts_distinct >> strip_tac
+      >> rpt scheme_env_tac
+      >> first_assum $ irule_at $ Pat `application _ _ _ _ = _`
+      >> first_assum $ irule_at $ Pos hd
+      >> gvs[Once valid_state_cases]
+      >> gvs[Once valid_cont_cases]
+      >> qrefine `SNOC front lst`
+      >> simp[SNOC_APPEND]
+      >> rpt $ irule_at Any EVERY2_REVERSE
+      >> first_assum $ irule_at $ Pos hd
+      >> irule EVERY2_MEM_MONO
+      >> first_assum $ irule_at $ Pat ‘LIST_REL _ _ _’
       >> qpat_x_assum ‘LIST_REL _ ts _’ $ assume_tac
       >> drule_then assume_tac EVERY2_LENGTH
       >> PairCases >> simp[]
       >> strip_tac
       >> drule_at_then (Pos last) assume_tac MEM_ZIP_MEM_MAP
       >> gvs[]
-      >> qsuff_tac ‘x0 ≠ t'’
+      >> qsuff_tac ‘x0 ≠ t''’
       >> strip_tac
       >> gvs[]
     )
@@ -2796,12 +1664,11 @@ Proof
 QED
 
 Theorem steps_preservation:
-  ∀ n store store' env env' e e' k k' (st : 'ffi state) mlenv var kv mle .
-  FUNPOW step n (store, k, env, e) = (store', k', env', e') ∧
-  valid_state store k env e ∧
+  ∀ n store store' e e' k k' (st : 'ffi state) mlenv var kv mle .
+  FUNPOW step n (store, k, e) = (store', k', e') ∧
+  valid_state store k e ∧
   cont_rel k kv ∧
-  e_ce_rel e var mlenv kv mle ∧
-  env_rel env mlenv ∧
+  cps_rel e var mlenv kv mle ∧
   LIST_REL store_entry_rel store st.refs
   ⇒
   ∃ ck st' mlenv' var' kv' mle' .
@@ -2809,10 +1676,9 @@ Theorem steps_preservation:
     =
     evaluate (st' with clock := start) mlenv' [mle']) ∧
     cont_rel k' kv' ∧
-    e_ce_rel e' var' mlenv' kv' mle' ∧
-    env_rel env' mlenv' ∧
+    cps_rel e' var' mlenv' kv' mle' ∧
     LIST_REL store_entry_rel store' st'.refs ∧
-    (¬ terminating_state (store', k', env', e') ⇒ n ≤ ck) ∧
+    (¬ terminating_state (store', k', e') ⇒ n ≤ ck) ∧
     st.ffi = st'.ffi
 Proof
   Induct >- (
@@ -2831,7 +1697,7 @@ Proof
   >> pop_assum $ drule_then assume_tac
   >> drule_all step_preservation
   >> rpt strip_tac
-  >> qpat_x_assum ‘∀ _ _ _ _ _ . _ ⇒ _’ drule_all
+  >> first_x_assum drule_all
   >> rpt strip_tac
   >> qexists ‘ck + ck'’
   >> gvs[SF SFY_ss]
@@ -2844,12 +1710,11 @@ Proof
 QED
 
 Theorem value_terminating:
-  ∀ n e v mle mlv store store' ks env (st:'ffi state) mlenv var kv .
-    FUNPOW step n (store, ks, env, e) = (store', [], FEMPTY, Val v) ∧
-    valid_state store ks env e ∧
-    e_ce_rel e var mlenv kv mle ∧
+  ∀ n e v mle mlv store store' ks (st:'ffi state) mlenv var kv .
+    FUNPOW step n (store, ks, e) = (store', [], Val v) ∧
+    valid_state store ks e ∧
+    cps_rel e var mlenv kv mle ∧
     cont_rel ks kv ∧
-    env_rel env mlenv ∧
     LIST_REL store_entry_rel store st.refs
     ⇒
     ∃ ck st' mlv . evaluate (st with clock:=ck) mlenv [mle]
@@ -2864,12 +1729,12 @@ Proof
   >> qexists ‘1 + ck’
   >> irule_at (Pos hd) EQ_TRANS
   >> pop_assum $ irule_at (Pos hd)
-  >> qpat_x_assum ‘_ (Val v) _ _ _ _’ mp_tac
-  >> simp[Once e_ce_rel_cases]
+  >> qpat_x_assum ‘cps_rel (Val v) _ _ _ _’ $ mp_tac
+    o SRULE [Once cps_rel_cases]
   >> rpt strip_tac
   >> gvs[]
-  >> qpat_x_assum ‘cont_rel [] _’ mp_tac
-  >> simp[Once cont_rel_cases]
+  >> qpat_x_assum ‘cont_rel [] _’ $ mp_tac
+    o SRULE [Once cont_rel_cases]
   >> rpt strip_tac
   >> gvs[]
   >> simp[evaluate_def, do_opapp_def, dec_clock_def]
@@ -2902,12 +1767,11 @@ Proof
 QED
 
 Theorem diverges:
-  ∀ e v mle mlv store store' ks env (st:'ffi state) mlenv var kv .
-    (∀ n . ¬ terminating_state (FUNPOW step n (store, ks, env, e))) ∧
-    valid_state store ks env e ∧
-    e_ce_rel e var mlenv kv mle ∧
+  ∀ e v mle mlv store store' ks (st:'ffi state) mlenv var kv .
+    (∀ n . ¬ terminating_state (FUNPOW step n (store, ks, e))) ∧
+    valid_state store ks e ∧
+    cps_rel e var mlenv kv mle ∧
     cont_rel ks kv ∧
-    env_rel env mlenv ∧
     LIST_REL store_entry_rel store st.refs
     ⇒
     ∀ ck . ∃ st' . evaluate (st with clock:=ck) mlenv [mle]
@@ -2916,13 +1780,13 @@ Theorem diverges:
 Proof
   rpt strip_tac
   >> last_x_assum $ qspec_then ‘ck’ assume_tac
-  >> Cases_on ‘FUNPOW step ck (store,ks,env,e)’
+  >> Cases_on ‘FUNPOW step ck (store,ks,e)’
   >> PairCases_on ‘r’
   >> drule_all steps_preservation
   >> rpt strip_tac
   >> gvs[]
-  >> qpat_x_assum ‘∀ _._=_’ $ qspec_then ‘0’ assume_tac
-  >> qpat_x_assum ‘e_ce_rel _ _ _ _ mle'’ $ assume_tac o SRULE [Once e_ce_rel_cases]
+  >> first_x_assum $ qspec_then ‘0’ assume_tac
+  >> qpat_x_assum ‘cps_rel _ _ _ _ mle'’ $ assume_tac o SRULE [Once cps_rel_cases]
   >> gvs[terminating_state_def]
   >> qpat_x_assum ‘cont_rel _ kv'’ $ assume_tac o SRULE [Once cont_rel_cases]
   >> qspecl_then [‘st' with clock:=0’,‘mlenv'’,‘e'’] mp_tac cps_val
